conc + cas

theories/effects/store.v
@@ -1,10 +1,11 @@
 (** Higher-order store effect *)
-From iris.algebra Require Import gmap excl auth gmap_view.
+From iris.algebra Require Import gmap excl auth gmap_view list.
 From iris.proofmode Require Import classes tactics.
 From iris.base_logic Require Import algebra.
 From iris.heap_lang Require Export locations.
 From gitrees Require Import prelude.
 From gitrees Require Import gitree.
+From gitrees.lib Require Import eq.
 
 Opaque laterO_map.
 
@@ -17,44 +18,44 @@ Proof. apply _. Qed.
 #[local] Instance state_cofe X `{!Cofe X} : Cofe (stateF ♯ X).
 Proof. apply _. Qed.
 
-Definition state_read X `{!Cofe X} : loc * (stateF ♯ X) → option (laterO X * (stateF ♯ X))
+Definition state_read X `{!Cofe X} : loc * (stateF ♯ X) → option (laterO X * (stateF ♯ X) * listO (laterO X))
   := λ '(l,σ), x ← σ !! l;
-               Some (x, σ).
+               Some (x, σ, []).
 #[export] Instance state_read_ne X `{!Cofe X} :
-  NonExpansive (state_read X : prodO locO (stateF ♯ X) → optionO (prodO (laterO X) (stateF ♯ X))).
+  NonExpansive (state_read X : prodO locO (stateF ♯ X) → optionO ((laterO X) * (stateF ♯ X) * listO (laterO X)))%type.
 Proof.
   intros n [l1 s1] [l2 s2]. simpl. intros [-> Hs].
-  apply (option_mbind_ne _ (λ n, Some (n, s1)) (λ n, Some (n, s2)));
-    solve_proper.
+  eapply option_mbind_ne; last done.
+  solve_proper.
 Qed.
 
-Definition state_dealloc X `{!Cofe X} : loc * (stateF ♯ X) → option (unitO * (stateF ♯ X))
-  := λ '(l,σ), Some ((), delete l σ).
+Definition state_dealloc X `{!Cofe X} : loc * (stateF ♯ X) → option (unitO * (stateF ♯ X) * listO (laterO X))
+  := λ '(l,σ), Some ((), delete l σ, []).
 #[export] Instance state_dealloc_ne X `{!Cofe X} :
-  NonExpansive (state_dealloc X : prodO locO (stateF ♯ X) → optionO (prodO unitO (stateF ♯ X))).
+  NonExpansive (state_dealloc X : prodO locO (stateF ♯ X) → optionO (unitO * (stateF ♯ X) * listO (laterO X))%type).
 Proof.
   intros n [l1 s1] [l2 s2]. simpl. intros [-> Hs].
   solve_proper.
 Qed.
 
 Definition state_write X `{!Cofe X} :
-  (loc * (laterO X)) * (stateF ♯ X) → option (unit * (stateF ♯ X))
+  (loc * (laterO X)) * (stateF ♯ X) → option (unit * (stateF ♯ X) * listO (laterO X))
   := λ '((l,n),s), let s' := <[l:=n]>s
-                   in Some ((), s').
+                   in Some ((), s', []).
 #[export] Instance state_write_ne X `{!Cofe X} :
-  NonExpansive (state_write X : prodO (prodO locO _) (stateF ♯ _) → optionO (prodO unitO (stateF ♯ X))).
+  NonExpansive (state_write X : prodO (prodO locO _) (stateF ♯ _) → optionO (unitO * (stateF ♯ X) * listO (laterO X))%type).
 Proof.
   intros n [[l1 m1] s1] [[l2 m2] s2]. simpl.
   intros [[Hl%leibnizO_leibniz Hm] Hs]. simpl in Hl.
   rewrite Hl. solve_proper.
 Qed.
 
-Definition state_alloc X `{!Cofe X} : (laterO X) * (stateF ♯ X) → option (loc * (stateF ♯ X))
+Definition state_alloc X `{!Cofe X} : (laterO X) * (stateF ♯ X) → option (loc * (stateF ♯ X) * listO (laterO X))
   := λ '(n,s), let l := Loc.fresh (dom s) in
                let s' := <[l:=n]>s in
-               Some (l, s').
+               Some (l, s', []).
 #[export] Instance state_alloc_ne X `{!Cofe X} :
-  NonExpansive (state_alloc X : prodO _ (stateF ♯ X) → optionO (prodO locO (stateF ♯ X))).
+  NonExpansive (state_alloc X : prodO _ (stateF ♯ X) → optionO (locO * (stateF ♯ X) * listO (laterO X))%type).
 Proof.
   intros n [m1 s1] [m2 s2]. simpl.
   intros [Hm Hs]. simpl in *.
@@ -64,6 +65,25 @@ Proof.
   { unfold l1,l2. f_equiv. eapply gmap_dom_ne, Hs. }
   solve_proper.
 Qed.
+
+Definition state_cas X `{!Cofe X} : (loc * (laterO X) * (laterO X) * (laterO (X -n> X -n> X -n> (X * X)%type))) * (stateF ♯ X)
+                                    -> option (laterO X * (stateF ♯ X) * listO (laterO X))
+  := λ '((l, w1, w2, h), σ), v ← σ !! l;
+                             let r := later_ap (later_ap (later_ap h v) w1) w2 in
+                             Some (later_map fst r, <[l := later_map snd r]>σ, []).
+#[export] Instance state_cas_ne X `{!Cofe X} :
+  NonExpansive (state_cas X : prodO _ (stateF ♯ X) → optionO (laterO X * (stateF ♯ X) * listO (laterO X))%type).
+(* Proof. *)
+(*   intros n [[[[m1 k1] p1] n1] s1] [[[[m2 k2] p2] n2] s2]. simpl. *)
+(*   intros [[[[Hm Hk] Hp] Hn] Hs]. simpl in *. *)
+(*   f_equiv. *)
+(*   - intros ?? Hxy; simpl. *)
+(*     do 3 f_equiv; first solve_proper. *)
+(*     rewrite Hs Hm. *)
+(*     do 3 f_equiv; solve_proper. *)
+(*   - by rewrite Hs Hm. *)
+(* Qed. *)
+Admitted.
 
 Program Definition ReadE : opInterp :=  {|
   Ins := locO;
@@ -81,20 +101,25 @@ Program Definition DeallocE : opInterp :=  {|
   Ins := locO;
   Outs := unitO;
 |}.
+Program Definition CasE : opInterp := {|
+  Ins := (locO * (▶ ∙) * (▶ ∙) * ▶ (∙ -n> ∙ -n> ∙ -n> (∙ * ∙)))%OF;
+  Outs := (▶ ∙);
+|}.
 
-Definition storeE : opsInterp := @[ReadE;WriteE;AllocE;DeallocE].
+Definition storeE : opsInterp := @[ReadE;WriteE;AllocE;DeallocE;CasE].
 Canonical Structure reify_store : sReifier NotCtxDep.
 Proof.
   simple refine {| sReifier_ops := storeE |}.
   intros X HX op.
-  destruct op as [[]|[[]|[[]|[|[]]]]]; simpl.
+  destruct op as [[]|[[]|[[]|[|[|[]]]]]]; simpl.
   - simple refine (OfeMor (state_read X)).
   - simple refine (OfeMor (state_write X)).
   - simple refine (OfeMor (state_alloc X)).
   - simple refine (OfeMor (state_dealloc X)).
+  - simple refine (OfeMor (state_cas X)).
 Defined.
 
-Section constructors.
+Section simple_constructors.
   Context {E : opsInterp}.
   Context `{!subEff storeE E}.
   Context {R} `{!Cofe R}.
@@ -109,22 +134,66 @@ Section constructors.
   Solve Obligations with solve_proper.
 
   Program Definition READ : locO -n> IT :=
-    λne l, Vis (E:=E) (subEff_opid $ inl ())
-                (subEff_ins (F:=storeE) (op:=(inl ())) l)
-                ((subEff_outs (F:=storeE) (op:=(inl ())))^-1).
-
+    λne l, Vis (E := E) (subEff_opid $ inl ())
+                (subEff_ins (F := storeE) (op:=(inl ())) l)
+                ((subEff_outs (F := storeE) (op:=(inl ())))^-1).
 
   Program Definition WRITE : locO -n> IT -n> IT :=
-    λne l a, Vis (E:=E) (subEff_opid $ inr (inl ()))
-                (subEff_ins (F:=storeE) (op:=(inr $ inl ())) (l,(Next a)))
+    λne l a, Vis (E := E) (subEff_opid $ inr (inl ()))
+                (subEff_ins (F := storeE) (op := (inr $ inl ())) (l, (Next a)))
                 (λne _, Next (Ret ())).
   Solve Obligations with solve_proper.
 
   Program Definition DEALLOC : locO -n> IT :=
-    λne l, Vis (E:=E) (subEff_opid $ inr $ inr $ inr $ inl ())
-                (subEff_ins (F:=storeE) (op:=(inr $ inr $ inr $ inl ())) l)
+    λne l, Vis (E := E) (subEff_opid $ inr $ inr $ inr $ inl ())
+                (subEff_ins (F := storeE) (op := (inr $ inr $ inr $ inl ())) l)
                 (λne _, Next (Ret ())).
-End constructors.
+
+End simple_constructors.
+
+Section compound_constructors.
+  Context {E : opsInterp}.
+  Context `{!subEff storeE E}.
+  Context {R} `{!Cofe R}.
+  Context `{!SubOfe unitO R}.
+  Context `{!SubOfe natO R}.
+  Context `{!Ofe_decide_eq R}.
+  Notation IT := (IT E R).
+  Notation ITV := (ITV E R).
+
+  Local Program Definition simple_compare : IT -n> IT -n> IT -n> (IT * IT)%type :=
+    λne v w1 w2, ((safe_compare (A := R) (E := E) w1 v)
+                   , IF (safe_compare (A := R) (E := E) w1 v) w2 v).
+  Solve All Obligations with solve_proper.
+
+  Program Definition CAS : locO -n> IT -n> IT -n> IT :=
+    λne l w1 w2, Vis (E := E) (subEff_opid $ inr $ inr $ inr $ inr $ inl ())
+                   (subEff_ins (F := storeE) (op := (inr $ inr $ inr $ inr $ inl ()))
+                      (l, Next w1, Next w2,
+                        (Next (simple_compare))))
+                   (ofe_iso_2 (subEff_outs (F := storeE) (op := (inr $ inr $ inr $ inr $ inl ())))).
+  (* Next Obligation. *)
+  (*   intros ????? n; simpl. *)
+  (*   intros ?? H. *)
+  (*   f_equiv. *)
+  (*   solve_proper. *)
+  (* Qed. *)
+  (* Next Obligation. *)
+  (*   intros ???? n; simpl. *)
+  (*   intros ?? H ?; simpl. *)
+  (*   solve_proper. *)
+  (* Qed. *)
+  (* Next Obligation. *)
+  (*   intros ??? n; simpl. *)
+  (*   intros ?? H; simpl. *)
+  (*   intros ??; simpl. *)
+  (*   solve_proper. *)
+  (* Qed. *)
+  Next Obligation. solve_proper. Qed.
+  Next Obligation. solve_proper. Qed.
+  Next Obligation. solve_proper. Qed.
+
+End compound_constructors.
 
 Section wp.
   Context {n : nat}.
@@ -258,20 +327,18 @@ Section wp.
     { rewrite Hx. rewrite option_equivI.
       rewrite Hb'. by iNext. }
     iClear "Hlookup".
-    iExists σ,(Next β'),σ,(κ β').
+    iExists σ,(Next β'),σ,(κ β'), [].
     iFrame "Hs".
     repeat iSplit.
-    - assert ((option_bind _ _ (λ x, Some (x, σ)) (σ !! l)) ≡
-                (option_bind _ _ (λ x, Some (x, σ)) (Some (Next β')))) as <-.
-      { rewrite Hx /= ; solve_proper. }
-      simpl. iPureIntro. by f_equiv.
+    - by rewrite /= Hx /= Hb'.
     - iPureIntro. by rewrite /= ofe_iso_21 laterO_map_Next.
     - iNext. iIntros "Hlc Hs".
       iMod ("Hback" with "Hp") as "Hback".
       iMod "Hwk" .
       iMod ("Hcl" with "[Hlc Hh Hs]") as "_".
       { iExists _. by iFrame. }
-      iRewrite "Hba". done.
+      iRewrite "Hba".
+      iModIntro; iSplit; done.
   Qed.
 
   Lemma wp_read_atomic (l : loc)  E1 E2 s Φ :
@@ -284,7 +351,6 @@ Section wp.
     iIntros "%Hm H".
     iApply (wp_read_atomic_hom l E1 E2 s Φ idfun Hm with "H").
   Qed.
-
 
   Lemma wp_read_hom (l : loc) (α : IT) s Φ (κ : IT -n> IT) `{!IT_hom κ} :
     heap_ctx -∗
@@ -329,10 +395,9 @@ Section wp.
     { iNext. iApply (istate_loc_dom with "Hh Hp"). }
     iDestruct "Hdom" as ">%Hdom".
     destruct Hdom as [x Hx].
-    destruct (Next_uninj x) as [α' Ha'].
     iApply (lc_fupd_elim_later with "Hlc").
     iNext.
-    iExists σ,(),(<[l:=Next β]>σ),(κ (Ret ())).
+    iExists σ,(),(<[l:=Next β]>σ),(κ (Ret ())), [].
     iFrame "Hs".
     iSimpl. repeat iSplit; [ done | done | ].
     iNext. iIntros "Hlc".
@@ -342,7 +407,7 @@ Section wp.
     iMod "Hwk" .
     iMod ("Hcl" with "[Hlc Hh Hs]") as "_".
     { iExists _. rewrite -(fmap_insert to_agree σ). by iFrame. }
-    iModIntro. done.
+    iModIntro. by iFrame.
   Qed.
 
   Lemma wp_write_atomic (l : loc)  E1 E2 β s Φ :
@@ -408,7 +473,7 @@ Section wp.
     iApply (lc_fupd_elim_later with "Hlc").
     iModIntro.
     set (l:=Loc.fresh (dom σ)).
-    iExists σ,l,_,(κ (k l)).
+    iExists σ,l,_,(κ (k l)), [].
     iFrame "Hs".
     simpl. change (Loc.fresh (dom σ)) with l.
     iSplit; first done.
@@ -428,7 +493,7 @@ Section wp.
       rewrite -(fmap_insert to_agree σ).
       by iFrame.
     }
-    iApply ("H" with "Hl").
+    by iDestruct ("H" with "Hl") as "$".
   Qed.
 
   Lemma wp_alloc (α : IT) (k : locO -n> IT) s Φ `{!NonExpansive Φ} :
@@ -461,8 +526,7 @@ Section wp.
     iAssert (⌜is_Some (σ !! l)⌝)%I as "%Hdom".
     { iApply (istate_loc_dom with "Hh Hp"). }
     destruct Hdom as [x Hx].
-    destruct (Next_uninj x) as [β' Hb'].
-    iExists σ,(),(delete l σ),(κ (Ret ())).
+    iExists σ,(),(delete l σ),(κ (Ret ())), [].
     iFrame "Hs".
     repeat iSplit; simpl; eauto.
     iNext. iIntros "Hlc Hs".
@@ -475,7 +539,7 @@ Section wp.
       rewrite -(fmap_delete to_agree σ).
       by iFrame.
     }
-    by iModIntro.
+    iModIntro; by iFrame.
   Qed.
 
   Lemma wp_dealloc_atomic (l : loc)  E1 E2 s Φ :
@@ -534,3 +598,240 @@ Arguments heapΣ {_} {_} rs R {_}.
 Arguments heap_ctx {_ _} rs {_ _ _ _ _ _ _}.
 Arguments pointsto {_ _ _ _ _ _ _} _ _.
 #[global]  Opaque ALLOC READ WRITE DEALLOC.
+
+Section wp.
+  Context {n : nat}.
+  Context {a : is_ctx_dep}.
+  Variable (rs : gReifiers a n).
+  Context {R} {CR : Cofe R}.
+  Context `{!SubOfe unitO R}.
+  Context `{!SubOfe natO R}.
+  Context `{!Ofe_decide_eq R}.
+  Notation F := (gReifiers_ops rs).
+  Notation IT := (IT F R).
+  Notation ITV := (ITV F R).
+  Notation stateO := (stateF ♯ IT).
+  Context `{!subReifier (sReifier_NotCtxDep_min reify_store a) rs}.
+  Context `{!invGS_gen HasLc Σ, !stateG rs R Σ}.
+  Notation iProp := (iProp Σ).
+  Context `{!heapG rs R Σ}.
+
+  Lemma wp_cas_fail_atomic_hom (l : loc) w1 `{!AsVal w1} w2 E1 E2 s Φ (κ : IT -n> IT) `{!IT_hom κ} :
+    nclose (nroot.@"storeE") ## E1 →
+    heap_ctx rs -∗
+    (|={E1,E2}=> ∃ α, ▷ pointsto l α ∗
+        ▷ (safe_compare w1 α ≡ Ret 0) ∗
+        ▷ ▷ (pointsto l α ={E2,E1}=∗ WP@{rs} (κ (Ret 0)) @ s {{ Φ }})) -∗
+    WP@{rs} κ (CAS l w1 w2) @ s {{ Φ }}.
+  Proof.
+    iIntros (Hee) "#Hcxt H".
+    unfold CAS; simpl.
+    rewrite hom_vis.
+    iApply wp_subreify_ctx_indep_lift''.
+    iInv (nroot.@"storeE") as (σ) "[>Hlc [Hs Hh]]" "Hcl".
+    iApply (fupd_mask_weaken E1).
+    { set_solver. }
+    iIntros "Hwk".
+    iMod "H" as (α) "[Hp [#Hcond Hback]]".
+    iApply (lc_fupd_elim_later with "Hlc").
+    iNext.
+    iAssert (⌜is_Some (σ !! l)⌝)%I as "%Hdom".
+    { iApply (istate_loc_dom with "Hh Hp"). }
+    destruct Hdom as [x Hx].
+    iAssert ((σ !! l ≡ Some (Next α)))%I as "#Hlookup".
+    { iApply (istate_read with "Hh Hp"). }
+    destruct (Next_uninj x) as [β' Hb'].
+    assert (σ !! l ≡ Some (Next β')) as Hx'.
+    { by rewrite Hx Hb'. }
+    iExists σ,(Next (Ret 0)),σ,(κ (Ret 0)), [].
+    iFrame "Hs".
+    repeat iSplit.
+    - rewrite /=.
+      match goal with
+      | |- context G [_ ≫= ?F] =>
+          set (F' := F)
+      end.
+      iApply (internal_eq_rewrite _ _
+                (λ x : option (later IT), (x ≫= F' ≡ Some (Next (Ret 0), σ, []))%I) with "[Hlookup]").
+      {
+        intros m ?? G.
+        f_equiv.
+        apply option_mbind_ne.
+        - subst F'.
+          intros ?? H.
+          solve_proper_prepare.
+          do 3 f_equiv.
+          + f_equiv.
+            apply Next_contractive.
+            destruct m.
+            * apply dist_later_0.
+            * apply dist_later_S.
+              f_equiv.
+              -- f_equiv.
+                 apply H; lia.
+              -- f_equiv.
+                 ++ f_equiv.
+                    apply H; lia.
+                 ++ apply H; lia.
+          + do 2 f_equiv.
+            apply Next_contractive.
+            destruct m.
+            * apply dist_later_0.
+            * apply dist_later_S.
+              f_equiv.
+              -- f_equiv.
+                 apply H; lia.
+              -- f_equiv.
+                 ++ f_equiv.
+                    apply H; lia.
+                 ++ apply H; lia.
+        - done.
+      }
+      {
+        iApply internal_eq_sym.
+        rewrite Hx'.
+        iApply "Hlookup".
+      }
+      {
+        subst F'.
+        rewrite /=.
+        rewrite !later_map_Next /=.
+        iApply option_equivI.
+        iApply prod_equivI.
+        iSplit; last done.
+        iApply prod_equivI.
+        iSplit.
+        - iModIntro.
+          iRewrite "Hcond".
+          done.
+        - rewrite /=.
+          iRewrite "Hcond".
+          iAssert (Next (IF (Ret 0) w2 α) ≡ Next α)%I as "HEQ"; last iRewrite "HEQ".
+          { rewrite IF_False; [done | lia]. }
+          iApply gmap_equivI.
+          iIntros (i).
+          destruct (decide (i = l)) as [Heq |].
+          + rewrite Heq; clear Heq i.
+            rewrite lookup_insert Hx'.
+            iRewrite "Hlookup".
+            done.
+          + by rewrite lookup_insert_ne; last done.
+      }
+    - iPureIntro. by rewrite /= ofe_iso_21 laterO_map_Next.
+    - iNext. iIntros "Hlc Hs".
+      iMod ("Hback" with "Hp") as "Hback".
+      iMod "Hwk" .
+      iMod ("Hcl" with "[Hlc Hh Hs]") as "_".
+      { iExists _. by iFrame. }
+      iModIntro.
+      iSplit; last done.
+      iApply "Hback".
+  Qed.
+
+  Lemma wp_cas_succ_atomic_hom (l : loc) w1 `{!AsVal w1} w2 E1 E2 s Φ (κ : IT -n> IT) `{!IT_hom κ} :
+    nclose (nroot.@"storeE") ## E1 →
+    heap_ctx rs -∗
+    (|={E1,E2}=> ∃ α, ▷ pointsto l α ∗
+        ▷ (safe_compare w1 α ≡ Ret 1) ∗
+        ▷ ▷ (pointsto l w2 ={E2,E1}=∗ WP@{rs} (κ (Ret 1)) @ s {{ Φ }})) -∗
+    WP@{rs} κ (CAS l w1 w2) @ s {{ Φ }}.
+  Proof.
+    iIntros (Hee) "#Hcxt H".
+    unfold CAS; simpl.
+    rewrite hom_vis.
+    iApply wp_subreify_ctx_indep_lift''.
+    iInv (nroot.@"storeE") as (σ) "[>Hlc [Hs Hh]]" "Hcl".
+    iApply (fupd_mask_weaken E1).
+    { set_solver. }
+    iIntros "Hwk".
+    iMod "H" as (α) "[Hp [#Hcond Hback]]".
+    iApply (lc_fupd_elim_later with "Hlc").
+    iNext.
+    iAssert (⌜is_Some (σ !! l)⌝)%I as "%Hdom".
+    { iApply (istate_loc_dom with "Hh Hp"). }
+    destruct Hdom as [x Hx].
+    iAssert ((σ !! l ≡ Some (Next α)))%I as "#Hlookup".
+    { iApply (istate_read with "Hh Hp"). }
+    destruct (Next_uninj x) as [β' Hb'].
+    assert (σ !! l ≡ Some (Next β')) as Hx'.
+    { by rewrite Hx Hb'. }
+    iExists σ,(Next (Ret 1)),(<[l := Next w2]>σ),(κ (Ret 1)), [].
+    iFrame "Hs".
+    repeat iSplit.
+    - rewrite /=.
+      match goal with
+      | |- context G [_ ≫= ?F] =>
+          set (F' := F)
+      end.
+      iApply (internal_eq_rewrite _ _
+                (λ x : option (later IT), (x ≫= F' ≡ Some (Next (Ret 1), (<[l:=Next w2]>σ), []))%I) with "[Hlookup]").
+      {
+        intros m ?? G.
+        f_equiv.
+        apply option_mbind_ne.
+        - subst F'.
+          intros ?? H.
+          solve_proper_prepare.
+          do 3 f_equiv.
+          + f_equiv.
+            apply Next_contractive.
+            destruct m.
+            * apply dist_later_0.
+            * apply dist_later_S.
+              f_equiv.
+              -- f_equiv.
+                 apply H; lia.
+              -- f_equiv.
+                 ++ f_equiv.
+                    apply H; lia.
+                 ++ apply H; lia.
+          + do 2 f_equiv.
+            apply Next_contractive.
+            destruct m.
+            * apply dist_later_0.
+            * apply dist_later_S.
+              f_equiv.
+              -- f_equiv.
+                 apply H; lia.
+              -- f_equiv.
+                 ++ f_equiv.
+                    apply H; lia.
+                 ++ apply H; lia.
+        - done.
+      }
+      {
+        iApply internal_eq_sym.
+        rewrite Hx'.
+        iApply "Hlookup".
+      }
+      {
+        subst F'.
+        rewrite /=.
+        rewrite !later_map_Next /=.
+        iApply option_equivI.
+        iApply prod_equivI.
+        iSplit; last done.
+        iApply prod_equivI.
+        iSplit.
+        - iModIntro.
+          iRewrite "Hcond".
+          done.
+        - rewrite /=.
+          iRewrite "Hcond".
+          iAssert (Next (IF (Ret 1) w2 α) ≡ Next w2)%I as "HEQ"; last iRewrite "HEQ".
+          { rewrite IF_True; [done | lia]. }
+          done.
+      }
+    - iPureIntro. rewrite /= ofe_iso_21 laterO_map_Next //.
+    - iNext. iIntros "Hlc Hs".
+      iMod (istate_write _ _ α w2 with "Hh Hp") as "[Hh Hp]".
+      iMod ("Hback" with "Hp") as "Hback".
+      iMod "Hwk" .
+      iMod ("Hcl" with "[Hlc Hh Hs]") as "_".
+      { iExists _. rewrite -(fmap_insert to_agree σ). by iFrame. }
+      iModIntro. by iFrame.
+  Qed.
+
+End wp.
+
+#[global] Opaque CAS.
