theories/gitree/reductions.v
@@ -1,9 +1,10 @@
 From iris.proofmode Require Import classes tactics.
 From iris.base_logic.lib Require Export invariants.
+From iris.algebra Require Import list.
 From gitrees Require Import prelude.
 From gitrees.gitree Require Import core reify.
 
-Section sstep.
+Section external_step.
   Context {A} `{!Cofe A} {a : is_ctx_dep}.
   Context (r : sReifier a).
   Notation F := (sReifier_ops r).
@@ -13,46 +14,127 @@ Section sstep.
   Notation stateO := (stateF ♯ IT).
 
   (** ** Reductions at the Prop level *)
-  Inductive sstep : IT → stateO → IT → stateO → Prop :=
-  | sstep_tick α β σ σ' :
+  Inductive external_step : IT → stateO → IT → stateO -> listO IT → Prop :=
+  | external_step_tick α β σ σ' :
     α ≡ Tick β →
     σ ≡ σ' →
-    sstep α σ β σ'
-  | sstep_reify α op i k β σ1 σ2 :
+    external_step α σ β σ' []
+  | external_step_reify α op i k β σ1 σ2 th :
     α ≡ Vis op i k →
-    reify r α σ1 ≡ (σ2, Tick β) →
-    sstep α σ1 β σ2.
-  #[export] Instance sstep_proper
-    : Proper ((≡) ==> (≡) ==> (≡) ==> (≡) ==> (iff)) sstep.
+    reify r α σ1 ≡ (σ2, Tick β, th) →
+    external_step α σ1 β σ2 th.
+
+  #[export] Instance external_step_proper
+    : Proper ((≡) ==> (≡) ==> (≡) ==> (≡) ==> (≡) ==> (iff)) external_step.
+  Proof.
+    intros α1 α2 Ha σ1 σ2 Hs β1 β2 Hb σ'1 σ'2 Hs' pool1 pool2 Hp.
+    simplify_eq/=. split.
+    - induction 1.
+      + inversion Hp; subst.
+        eapply external_step_tick.
+        ++ rewrite -Ha -Hb//.
+        ++ rewrite -Hs' -Hs//.
+      + eapply external_step_reify.
+        ++ rewrite -Ha//.
+        ++ rewrite -Hb -Hs' -Hs -Hp //.
+           rewrite -H0. repeat f_equiv; eauto.
+    - induction 1.
+      + inversion Hp; subst.
+        eapply external_step_tick.
+        ++ rewrite Ha Hb//.
+        ++ rewrite Hs' Hs//.
+      + eapply external_step_reify.
+        ++ rewrite Ha//.
+        ++ rewrite Hb Hs' Hs Hp //.
+           rewrite -H0. repeat f_equiv; eauto.
+  Qed.
+
+  Inductive external_steps : IT → stateO → IT → stateO -> listO IT → nat → Prop :=
+  | steps_zero α β σ σ' l : α ≡ β → σ ≡ σ' → l ≡ [] → external_steps α σ β σ' l 0
+  | steps_many α1 σ1 α2 σ2 α3 σ3 l1 l2 l3 n2 :
+    l3 ≡ l1 ++ l2 →
+    external_step α1 σ1 α2 σ2 l1 →
+    external_steps α2 σ2 α3 σ3 l2 n2 →
+    external_steps α1 σ1 α3 σ3 l3 (S n2).
+
+  #[export] Instance external_steps_proper
+    : Proper ((≡) ==> (≡) ==> (≡) ==> (≡) ==> (≡) ==> (=) ==> (iff)) external_steps.
+  Proof.
+    intros α α' Ha σ σ' Hs β β' Hb σ2 σ2' Hs2 l1 l2 Hl n1 n2 Hnm.
+    fold_leibniz. simplify_eq /=.
+    split.
+    - intro HS. revert α' β' σ' σ2' Ha Hb Hs Hs2 l2 Hl.
+      induction HS=>α' β' σ'' σ2' Ha Hb Hs Hs2 l2' Hl.
+      + constructor.
+        ++ rewrite -Ha -Hb //.
+        ++ rewrite -Hs -Hs2 //.
+        ++ rewrite -Hl H1 //.
+      + econstructor; last first.
+        ++ eapply IHHS; eauto.
+        ++ rewrite -Ha -Hs //.
+        ++ rewrite -Hl H //.
+    - intro HS. revert α β σ σ2 Ha Hb Hs Hs2 l1 Hl.
+      induction HS=>α' β' σ'' σ2' Ha Hb Hs Hs2 l1' Hl.
+      + constructor.
+        ++ rewrite Ha Hb //.
+        ++ rewrite Hs Hs2 //.
+        ++ rewrite Hl -H1 //.
+      + econstructor; last first.
+        ++ eapply IHHS; eauto.
+        ++ rewrite Ha Hs //.
+        ++ rewrite Hl -H //.
+  Qed.
+
+  Inductive tp_external_step : listO IT → stateO → listO IT → stateO → Prop :=
+  | tp_external_step_atomic ρ1 ρ2 s1 s2 e1 e2 t1 t2 en :
+    ρ1 ≡ (t1 ++ e1 :: t2) →
+    ρ2 ≡ (t1 ++ e2 :: t2 ++ en) →
+    external_step e1 s1 e2 s2 en  →
+    tp_external_step ρ1 s1 ρ2 s2.
+
+  #[export] Instance tp_external_step_proper
+    : Proper ((≡) ==> (≡) ==> (≡) ==> (≡) ==> (iff)) tp_external_step.
   Proof.
     intros α1 α2 Ha σ1 σ2 Hs β1 β2 Hb σ'1 σ'2 Hs'.
     simplify_eq/=. split.
     - induction 1.
-      + eapply sstep_tick.
-        ++ rewrite -Ha -Hb//.
-        ++ rewrite -Hs' -Hs//.
-      + eapply sstep_reify.
-        ++ rewrite -Ha//.
-        ++ rewrite -Hb -Hs' -Hs//.
-           rewrite -H0. repeat f_equiv; eauto.
+      + eapply tp_external_step_atomic.
+        ++ rewrite -Ha //.
+        ++ rewrite -Hb //.
+        ++ rewrite -Hs -Hs' //.
     - induction 1.
-      + eapply sstep_tick.
-        ++ rewrite Ha Hb//.
-        ++ rewrite Hs' Hs//.
-      + eapply sstep_reify.
-        ++ rewrite Ha//.
-        ++ rewrite Hb Hs' Hs//.
-           rewrite -H0. repeat f_equiv; eauto.
+      + eapply tp_external_step_atomic.
+        ++ rewrite Ha //.
+        ++ rewrite Hb //.
+        ++ rewrite Hs Hs' //.
   Qed.
 
-  Inductive ssteps : IT → stateO → IT → stateO → nat → Prop :=
-  | ssteps_zero α β σ σ' : α ≡ β → σ ≡ σ' → ssteps α σ β σ' 0
-  | ssteps_many α1 σ1 α2 σ2 α3 σ3 n2 :
-    sstep α1 σ1 α2 σ2 →
-    ssteps α2 σ2 α3 σ3 n2 →
-    ssteps α1 σ1 α3 σ3 (1+n2).
-  #[export] Instance ssteps_proper
-    : Proper ((≡) ==> (≡) ==> (≡) ==> (≡) ==> (=) ==> (iff)) ssteps.
+  Lemma external_step_tp_external_step α β σ σ' e1 e2 l
+    : external_step α σ β σ' l
+      → tp_external_step (e1 ++ α :: e2) σ (e1 ++ β :: e2 ++ l) σ'.
+  Proof.
+    induction 1 as [???? H1 H2| ???????? H1 H2].
+    - econstructor 1; first reflexivity; first last.
+      + rewrite H1.
+        by constructor.
+      + by rewrite app_nil_r.
+    - econstructor 1; first reflexivity; first last.
+      + rewrite H1.
+        econstructor 2; first done.
+        setoid_replace (reify r (Vis op i k) σ1) with (reify r α σ1); first done.
+        do 2 f_equiv; by symmetry.
+      + reflexivity.
+  Qed.
+
+  Inductive tp_external_steps : listO IT → stateO → listO IT → stateO → nat → Prop :=
+  | tp_steps_zero α β σ σ' : α ≡ β → σ ≡ σ' → tp_external_steps α σ β σ' 0
+  | tp_steps_many α1 σ1 α2 σ2 α3 σ3 n2 :
+    tp_external_step α1 σ1 α2 σ2 →
+    tp_external_steps α2 σ2 α3 σ3 n2 →
+    tp_external_steps α1 σ1 α3 σ3 (S n2).
+
+  #[export] Instance tp_external_steps_proper
+    : Proper ((≡) ==> (≡) ==> (≡) ==> (≡) ==> (=) ==> (iff)) tp_external_steps.
   Proof.
     intros α α' Ha σ σ' Hs β β' Hb σ2 σ2' Hs2 n1 n2 Hnm.
     fold_leibniz. simplify_eq/=.
@@ -75,17 +157,51 @@ Section sstep.
         ++ rewrite Ha Hs//.
   Qed.
 
-  Lemma ssteps_tick_n n α σ : ssteps (Tick_n n α) σ α σ n.
+  Lemma external_steps_tp_external_steps α β σ σ' e1 e2 l n
+    : external_steps α σ β σ' l n
+      → tp_external_steps (e1 ++ α :: e2) σ (e1 ++ β :: e2 ++ l) σ' n.
+  Proof.
+    intros H.
+    revert e2.
+    induction H as [ ????? H1 H2 H3 | ?????????? H1 H2 H3 IH]; intros e2.
+    - rewrite H1 H2 H3 app_nil_r.
+      by constructor.
+    - econstructor.
+      + by apply external_step_tp_external_step.
+      + rewrite H1.
+        specialize (IH (e2 ++ l1)).
+        rewrite -app_assoc in IH.
+        apply IH.
+  Qed.
+
+  Lemma external_steps_tick_n n α σ
+    : external_steps (Tick_n n α) σ α σ [] n.
   Proof.
     induction n; first by constructor.
     change (S n) with (1+n).
     change (Tick_n (1+n) α) with (Tick $ Tick_n n α).
     econstructor; last eassumption.
-    econstructor; reflexivity.
+    { rewrite app_nil_r; reflexivity. }
+    by econstructor.
   Qed.
-End sstep.
 
-Section istep.
+  Lemma tp_external_steps_tick_n p1 p2 n α σ
+    : tp_external_steps (p1 ++ (Tick_n n α) :: p2) σ (p1 ++ α :: p2) σ n.
+  Proof.
+    induction n; first by constructor.
+    change (S n) with (1+n).
+    change (Tick_n (1+n) α) with (Tick $ Tick_n n α).
+    econstructor; last eassumption.
+    apply (tp_external_step_atomic (p1 ++ Tick (Tick_n n α) :: p2)
+             (p1 ++ Tick_n n α :: p2)
+             σ σ (Tick (Tick_n n α)) (Tick_n n α) p1 p2 []
+             (reflexivity _)).
+    - by rewrite app_nil_r.
+    - by constructor.
+  Qed.
+End external_step.
+
+Section internal_step.
   Context {A} `{!Cofe A} {a : is_ctx_dep}.
   Context (r : sReifier a).
   Notation F := (sReifier_ops r).
@@ -97,84 +213,228 @@ Section istep.
   Context `{!invGS_gen hlc Σ}.
   Notation iProp := (iProp Σ).
 
-  Program Definition istep :
-    IT -n> stateO -n> IT -n> stateO -n> iProp :=
-    λne α σ β σ', ((α ≡ Tick β ∧ σ ≡ σ')
-                   ∨ (∃ op i k, α ≡ Vis op i k ∧ reify r α σ ≡ (σ', Tick β)))%I.
+  Program Definition internal_step :
+    IT -n> stateO -n> IT -n> stateO -n> listO IT -n> iProp :=
+    λne α σ β σ' en, ((α ≡ Tick β ∧ σ ≡ σ' ∧ en ≡ [])
+                     ∨ (∃ op i k,
+                          α ≡ Vis op i k
+                          ∧ reify r α σ ≡ (σ', Tick β, en)))%I.
   Solve All Obligations with solve_proper.
 
-  Program Definition isteps_pre
-    (self : IT -n> stateO -n> IT -n> stateO -n> natO -n> iProp):
-    IT -n> stateO -n> IT -n> stateO -n> natO -n> iProp :=
-    λne α σ β σ' n, ((n ≡ 0 ∧ α ≡ β ∧ σ ≡ σ')
-                     ∨ (∃ n' α0 σ0, n ≡ (1+n') ∧ istep α σ α0 σ0 ∧
-                                      ▷ self α0 σ0 β σ' n'))%I.
+  Program Definition internal_steps_pre
+    (self : IT -n> stateO -n> IT -n> stateO -n> listO IT -n> natO -n> iProp):
+    IT -n> stateO -n> IT -n> stateO -n> listO IT -n> natO -n> iProp :=
+    λne α σ β σ'' l n, ((n ≡ 0 ∧ α ≡ β ∧ σ ≡ σ'' ∧ l ≡ [])
+                        ∨ (∃ n' γ σ' l' l'',
+                             l ≡ l' ++ l''
+                             ∧ n ≡ (S n')
+                             ∧ internal_step α σ γ σ' l'
+                             ∧ ▷ self γ σ' β σ'' l'' n'))%I.
   Solve All Obligations with solve_proper.
 
-  Global Instance isteps_pre_ne : NonExpansive isteps_pre.
+  Global Instance internal_steps_pre_ne : NonExpansive internal_steps_pre.
   Proof. solve_proper. Qed.
-  Global Instance isteps_pre_contractive : Contractive isteps_pre.
+  Global Instance internal_steps_pre_contractive
+    : Contractive internal_steps_pre.
   Proof. solve_contractive. Qed.
-  Definition isteps : IT -n> stateO -n> IT -n> stateO -n> natO -n> iProp
-    := fixpoint isteps_pre.
+  Definition internal_steps
+    : IT -n> stateO -n> IT -n> stateO -n> listO IT -n> natO -n> iProp
+    := fixpoint internal_steps_pre.
 
-  Lemma isteps_unfold α β σ σ' n :
-    isteps α σ β σ' n ≡
-      ((n ≡ 0 ∧ α ≡ β ∧ σ ≡ σ')
-       ∨ (∃ n' α0 σ0, n ≡ (1+n') ∧ istep α σ α0 σ0 ∧
-                        ▷ isteps α0 σ0 β σ' n'))%I.
-  Proof. unfold isteps. apply (fixpoint_unfold isteps_pre _ _ _ _ _) . Qed.
-
+  Lemma internal_steps_unfold α β σ σ'' n l :
+    internal_steps α σ β σ'' l n ≡
+      ((n ≡ 0 ∧ α ≡ β ∧ σ ≡ σ'' ∧ l ≡ [])
+       ∨ (∃ n' γ σ' l' l'',
+            l ≡ l' ++ l''
+            ∧ n ≡ (S n')
+            ∧ internal_step α σ γ σ' l'
+            ∧ ▷ internal_steps γ σ' β σ'' l'' n'))%I.
+  Proof.
+    unfold internal_steps.
+    apply (fixpoint_unfold internal_steps_pre _ _ _ _ _) .
+  Qed.
 
   (** Properties *)
-  Lemma isteps_0 α β σ σ' :
-    isteps α σ β σ' 0 ≡ (α ≡ β ∧ σ ≡ σ')%I.
+  Lemma internal_steps_0 α β σ σ' l :
+    internal_steps α σ β σ' l 0 ≡ (α ≡ β ∧ σ ≡ σ' ∧ l ≡ [])%I.
   Proof.
-    rewrite isteps_unfold. iSplit.
+    rewrite internal_steps_unfold. iSplit.
+    - iDestruct 1 as "[(_ & $ & $)|H]".
+      iExFalso.
+      iDestruct "H" as (n' ? ? ?) "[% [_ [%HH _]]]".
+      fold_leibniz. lia.
+    - iDestruct 1 as "[H1 H2]". iLeft; eauto.
+  Qed.
+
+  Lemma internal_steps_S α β σ σ'' l k :
+    internal_steps α σ β σ'' l (S k) ≡
+      (∃ γ σ' l' l'',
+         l ≡ l' ++ l''
+         ∧ internal_step α σ γ σ' l'
+         ∧ ▷ internal_steps γ σ' β σ'' l'' k)%I.
+  Proof.
+    rewrite internal_steps_unfold. iSplit.
+    - iDestruct 1 as "[(% & _ & _)|H]"; first by fold_leibniz; lia.
+      iDestruct "H" as (n' ? ? ? ?) "(H1 & [% (H2 & H3)])".
+      fold_leibniz. assert (k = n') as -> by lia.
+      iExists _,_,_. eauto with iFrame.
+    - iDestruct 1 as (γ σ' l' l'') "[H1 [H2 H3]]".
+      iRight.
+      iExists k,γ,σ',l',l''.
+      eauto with iFrame.
+  Qed.
+
+  Program Definition tp_internal_step :
+    listO IT -n> stateO -n> listO IT -n> stateO -n> iProp :=
+    λne α σ β σ', (∃ α0 α1 γ γ' en,
+                    α ≡ (α0 ++ γ :: α1)
+                    ∧ β ≡ (α0 ++ γ' :: α1 ++ en)
+                    ∧ internal_step γ σ γ' σ' en)%I.
+  Solve All Obligations with solve_proper.
+
+  Global Instance tp_internal_step_ne : NonExpansive tp_internal_step.
+  Proof. solve_proper. Qed.
+
+  Program Definition tp_internal_steps_pre
+    (self : listO IT -n> stateO -n> listO IT -n> stateO -n> natO -n> iProp):
+    listO IT -n> stateO -n> listO IT -n> stateO -n> natO -n> iProp :=
+    λne α σ β σ'' n, ((n ≡ 0 ∧ α ≡ β ∧ σ ≡ σ'')
+                     ∨ (∃ n' γ σ',
+                          n ≡ (S n')
+                          ∧ tp_internal_step α σ γ σ'
+                          ∧ ▷ self γ σ' β σ'' n'))%I.
+  Solve All Obligations with solve_proper.
+
+  Global Instance tp_internal_steps_pre_ne : NonExpansive tp_internal_steps_pre.
+  Proof. solve_proper. Qed.
+  Global Instance tp_internal_steps_pre_contractive
+    : Contractive tp_internal_steps_pre.
+  Proof. solve_contractive. Qed.
+  Definition tp_internal_steps
+    : listO IT -n> stateO -n> listO IT -n> stateO -n> natO -n> iProp
+    := fixpoint tp_internal_steps_pre.
+
+  Lemma tp_internal_steps_unfold α β σ σ'' n :
+    tp_internal_steps α σ β σ'' n ≡
+      ((n ≡ 0 ∧ α ≡ β ∧ σ ≡ σ'')
+       ∨ (∃ n' γ σ',
+            n ≡ (S n')
+            ∧ tp_internal_step α σ γ σ'
+            ∧ ▷ tp_internal_steps γ σ' β σ'' n'))%I.
+  Proof.
+    unfold tp_internal_steps.
+    apply (fixpoint_unfold tp_internal_steps_pre _ _ _ _ _) .
+  Qed.
+
+  (** Properties *)
+  Lemma tp_internal_steps_0 α β σ σ' :
+    tp_internal_steps α σ β σ' 0 ≡ (α ≡ β ∧ σ ≡ σ')%I.
+  Proof.
+    rewrite tp_internal_steps_unfold. iSplit.
     - iDestruct 1 as "[(_ & $ & $)|H]".
       iExFalso.
       iDestruct "H" as (n' ? ?) "[% HH]".
       fold_leibniz. lia.
     - iDestruct 1 as "[H1 H2]". iLeft; eauto.
   Qed.
-  Lemma isteps_S α β σ σ' k :
-    isteps α σ β σ' (S k) ≡ (∃ α1 σ1, istep α σ α1 σ1 ∧ ▷ isteps α1 σ1 β σ' k)%I.
+
+  Lemma tp_internal_steps_S α β σ σ'' k :
+    tp_internal_steps α σ β σ'' (S k) ≡ (∃ γ σ',
+                                tp_internal_step α σ γ σ'
+                                ∧ ▷ tp_internal_steps γ σ' β σ'' k)%I.
   Proof.
-    rewrite isteps_unfold. iSplit.
+    rewrite tp_internal_steps_unfold. iSplit.
     - iDestruct 1 as "[(% & _ & _)|H]"; first by fold_leibniz; lia.
       iDestruct "H" as (n' ? ?) "[% HH]".
+      iDestruct "HH" as "(H1 & H2)".
       fold_leibniz. assert (k = n') as -> by lia.
       iExists _,_. eauto with iFrame.
-    - iDestruct 1 as (α1 σ1) "[H1 H2]".
-      iRight. iExists k,α1,σ1. eauto with iFrame.
-  Qed.
-  #[export] Instance isteps_persistent α σ β σ' k : Persistent (isteps α σ β σ' k).
-  Proof.
-    revert α σ. induction k as [|k]=> α σ.
-    - rewrite isteps_0. apply _.
-    - rewrite isteps_S. apply _.
+    - iDestruct 1 as (γ σ') "[H1 H2]".
+      iRight.
+      iExists k,γ,σ'.
+      eauto with iFrame.
   Qed.
 
-  Lemma sstep_istep α β σ σ' :
-    sstep r α σ β σ' → (⊢ istep α σ β σ').
+  #[export] Instance internal_step_persistent α σ β σ' en
+    : Persistent (internal_step α σ β σ' en).
+  Proof. apply _. Qed.
+
+  #[export] Instance internal_steps_persistent α σ β σ' en k
+    : Persistent (internal_steps α σ β σ' en k).
+  Proof.
+    revert α σ en. induction k as [|k]=> α σ en.
+    - rewrite internal_steps_0. apply _.
+    - rewrite internal_steps_S. apply _.
+  Qed.
+
+  #[export] Instance tp_internal_step_persistent α σ β σ'
+    : Persistent (tp_internal_step α σ β σ').
+  Proof. apply _. Qed.
+
+  #[export] Instance tp_internal_steps_persistent α σ β σ' k
+    : Persistent (tp_internal_steps α σ β σ' k).
+  Proof.
+    revert α σ. induction k as [|k]=> α σ.
+    - rewrite tp_internal_steps_0. apply _.
+    - rewrite tp_internal_steps_S. apply _.
+  Qed.
+
+  Lemma tp_internal_step_decomp α β σ σ' :
+    ⊢ tp_internal_step α σ β σ' -∗ ∃ β1 β2 : listO IT, β ≡ β1 ++ β2 ∗ length α ≡ length β1.
+  Proof.
+    iIntros "H".
+    iDestruct "H" as "(%a1 & %a2 & %b1 & %b2 & %c3 & H1 & H2 & H3)".
+    iExists (a1 ++ b2 :: a2), c3.
+    iSplit.
+    - rewrite app_comm_cons.
+      by rewrite -app_assoc.
+    - iRewrite "H1".
+      rewrite !app_length //.
+  Qed.
+
+  Lemma external_step_internal_step α β σ σ' en :
+    external_step r α σ β σ' en → (⊢ internal_step α σ β σ' en).
   Proof.
     inversion 1; simplify_eq/=.
     - iLeft. eauto.
     - iRight. iExists _,_,_. iSplit; eauto.
   Qed.
-  Lemma ssteps_isteps α β σ σ' n :
-    ssteps r α σ β σ' n → (⊢ isteps α σ β σ' n).
+
+  Lemma external_steps_internal_steps α β σ σ' en k :
+    external_steps r α σ β σ' en k → (⊢ internal_steps α σ β σ' en k).
   Proof.
-    revert α σ. induction n=> α σ; inversion 1; simplify_eq /=.
-    - rewrite isteps_unfold. iLeft. eauto.
-    - rewrite isteps_unfold. iRight. iExists n, α2,σ2.
-      repeat iSplit; eauto.
-      + iApply sstep_istep; eauto.
-      + iNext. iApply IHn; eauto.
+    induction 1.
+    - by iApply internal_steps_0.
+    - iApply internal_steps_S.
+      iExists _,_,_,_; iSplit; first done.
+      iSplit; [by iApply external_step_internal_step | by iNext].
+  Qed.
+
+  Lemma tp_external_step_tp_internal_step α β σ σ' :
+    tp_external_step r α σ β σ' → (⊢ tp_internal_step α σ β σ').
+  Proof.
+    inversion 1 as [????????? H1 H2 H3]; simplify_eq.
+    iPoseProof (external_step_internal_step e1 e2 σ σ' en H3) as "H".
+    iExists _, _, _, _, _.
+    iSplit; first eauto.
+    iSplit; first eauto.
+    done.
+  Qed.
+
+  Lemma tp_external_steps_tp_internal_steps α β σ σ' n :
+    tp_external_steps r α σ β σ' n → (⊢ tp_internal_steps α σ β σ' n).
+  Proof.
+    revert α σ. induction n as [| ? IH] => α σ; inversion 1; simplify_eq /=.
+    - rewrite tp_internal_steps_unfold. iLeft. eauto.
+    - rewrite tp_internal_steps_unfold. iRight. iExists n, _, _.
+      iSplit; first eauto.
+      iSplit.
+      + iApply tp_external_step_tp_internal_step; eauto.
+      + iNext. iApply IH; eauto.
   Qed.
 
   Local Lemma tick_safe_externalize (α : IT) σ :
-    (⊢ ∃ β σ', α ≡ Tick β ∧ σ ≡ σ' : iProp) → ∃ β σ', sstep r α σ β σ'.
+    (⊢ ∃ β σ', α ≡ Tick β ∧ σ ≡ σ' : iProp) → ∃ β σ', external_step r α σ β σ' [].
   Proof.
     intros Hprf.
     destruct (IT_dont_confuse α)
@@ -201,76 +461,119 @@ Section istep.
 
   (* ctx-free steps *)
   Local Lemma effect_safe_externalize (α : IT) σ :
-    (⊢ ∃ β σ', (∃ op i k, α ≡ Vis op i k ∧ reify r α σ ≡ (σ', Tick β)) : iProp) →
-    ∃ β σ', sstep r α σ β σ'.
+    (⊢ ∃ β σ' en, (∃ op i k, α ≡ Vis op i k ∧ reify r α σ ≡ (σ', Tick β, en)) : iProp) →
+    ∃ β σ' en, external_step r α σ β σ' en.
   Proof.
     intros Hprf.
     destruct (IT_dont_confuse α)
       as [[e Ha] | [[n Ha] | [ [g Ha] | [[α' Ha]|[op [i [k Ha]]]] ]]].
     + exfalso. eapply uPred.pure_soundness.
       iPoseProof (Hprf) as "H".
-      iDestruct "H" as (β σ' op i k) "[Ha _]". rewrite Ha.
+      iDestruct "H" as (β σ' en op i k) "[Ha _]". rewrite Ha.
       iApply (IT_vis_err_ne). iApply internal_eq_sym.
       by iApply "Ha".
     + exfalso. eapply uPred.pure_soundness.
       iPoseProof (Hprf) as "H".
-      iDestruct "H" as (β σ' op i k) "[Ha _]". rewrite Ha.
+      iDestruct "H" as (β σ' en op i k) "[Ha _]". rewrite Ha.
       iApply (IT_ret_vis_ne with "Ha").
     + exfalso. eapply uPred.pure_soundness.
       iPoseProof (Hprf) as "H".
-      iDestruct "H" as (β σ' op i k) "[Ha _]". rewrite Ha.
+      iDestruct "H" as (β σ' en op i k) "[Ha _]". rewrite Ha.
       iApply (IT_fun_vis_ne with "Ha").
     + exfalso. eapply uPred.pure_soundness.
       iPoseProof (Hprf) as "H".
-      iDestruct "H" as (β σ' op i k) "[Ha _]". rewrite Ha.
+      iDestruct "H" as (β σ' en op i k) "[Ha _]". rewrite Ha.
       iApply (IT_tick_vis_ne with "Ha").
-    + destruct (reify r (Vis op i k) σ) as [σ1 α1] eqn:Hr.
+    + destruct (reify r (Vis op i k) σ) as [[σ1 α1] en] eqn:Hr.
       assert ((∃ α' : IT, α1 ≡ Tick α') ∨ (α1 ≡ Err RuntimeErr)) as [[α' Ha']| Ha'].
       { eapply (reify_is_always_a_tick r op i k σ).
         by rewrite Hr.
       }
-      * exists α',σ1. eapply sstep_reify; eauto.
+      * exists α',σ1, en. eapply external_step_reify; eauto.
         rewrite -Ha' -Hr; repeat f_equiv; eauto.
       * exfalso. eapply uPred.pure_soundness.
         iPoseProof (Hprf) as "H".
-        iDestruct "H" as (β σ' op' i' k') "[_ Hb]".
+        iDestruct "H" as (β σ' en' op' i' k') "[_ Hb]".
         assert (reify r (Vis op i k) σ ≡ reify r α σ) as Har.
         { f_equiv. by rewrite Ha. }
         iEval (rewrite -Har) in "Hb".
         iEval (rewrite Hr) in "Hb".
-        iPoseProof (prod_equivI with "Hb") as "[_ Hb']".
+        iPoseProof (prod_equivI with "Hb") as "[Hb'' Hb']".
+        iPoseProof (prod_equivI with "Hb''") as "[_ Hb'''']".
         simpl. rewrite Ha'.
-        iApply (IT_tick_err_ne). iApply (internal_eq_sym with "Hb'").
+        iApply (IT_tick_err_ne). iApply (internal_eq_sym with "Hb''''").
   Qed.
 
-  Local Lemma istep_safe_disj α σ :
-    (∃ β σ', istep α σ β σ')
+  Local Lemma internal_step_safe_disj α σ :
+    (∃ β σ' en, internal_step α σ β σ' en)
     ⊢ (∃ β σ', α ≡ Tick β ∧ σ ≡ σ')
-      ∨ (∃ β σ', (∃ op i k, α ≡ Vis op i k ∧ reify r α σ ≡ (σ', Tick β))).
+      ∨ (∃ β σ' en, (∃ op i k, α ≡ Vis op i k ∧ reify r α σ ≡ (σ', Tick β, en))).
   Proof.
     rewrite -bi.or_exist.
     apply bi.exist_mono=>β.
-    rewrite -bi.or_exist//.
+    rewrite -bi.or_exist.
+    rewrite /internal_step /=.
+    iIntros "(%σ' & %en & [(H1 & H2 & H3) | H])".
+    - iExists σ'; iLeft; by iFrame.
+    - iExists σ'; iRight; by iExists en.
+  Qed.
+
+  Lemma internal_step_tp_internal_step α β σ σ' e1 e2 l
+    : ⊢ internal_step α σ β σ' l
+      → tp_internal_step (e1 ++ α :: e2) σ (e1 ++ β :: e2 ++ l) σ'.
+  Proof.
+    iStartProof.
+    iIntros "H".
+    iExists e1, e2, α, β, l.
+    iSplit; first done.
+    iSplit; first done.
+    done.
+  Qed.
+
+  Lemma internal_steps_tp_internal_steps α β σ σ' e1 e2 l n
+    : ⊢ internal_steps α σ β σ' l n
+      → tp_internal_steps (e1 ++ α :: e2) σ (e1 ++ β :: e2 ++ l) σ' n.
+  Proof.
+    iStartProof.
+    iLöb as "IH" forall (l e2 n α σ).
+    iIntros "H".
+    rewrite internal_steps_unfold.
+    iDestruct "H" as "[(H1 & H2 & H3 & H4)
+        |(%n' & %γ & %σ'' & %l' & %l'' & H1 & H2 & H3 & H4)]".
+    - iRewrite "H1"; iRewrite "H2"; iRewrite "H3"; iRewrite "H4".
+      iApply tp_internal_steps_0.
+      by rewrite app_nil_r.
+    - iRewrite "H1"; iRewrite "H2".
+      iApply tp_internal_steps_S.
+      iExists (e1 ++ γ :: e2 ++ l'), σ''.
+      iSplit.
+      + by iApply internal_step_tp_internal_step.
+      + iNext.
+        iSpecialize ("IH" $! l'' (e2 ++ l') n' γ σ'').
+        rewrite app_assoc.
+        by iApply "IH".
   Qed.
 
   (* this is true only for iProp/uPred? *)
   Definition disjunction_property (P Q : iProp) := (⊢ P ∨ Q) → (⊢ P) ∨ (⊢ Q).
 
-  Lemma istep_safe_sstep α σ :
+  Lemma internal_step_safe_external_step α σ :
     (∀ P Q, disjunction_property P Q) →
-    (⊢ ∃ β σ', istep α σ β σ') → ∃ β σ', sstep r α σ β σ'.
+    (⊢ ∃ β σ' en, internal_step α σ β σ' en) → ∃ β σ' en, external_step r α σ β σ' en.
   Proof.
     intros Hdisj.
-    rewrite istep_safe_disj.
+    rewrite internal_step_safe_disj.
     intros [H|H]%Hdisj.
-    - by apply tick_safe_externalize.
-    - by apply effect_safe_externalize.
+    - pose proof (tick_safe_externalize _ _ H) as [β [σ' G]].
+      by exists β, σ', [].
+    - pose proof (effect_safe_externalize _ _ H) as [β [σ' [en G]]].
+      by exists β, σ', en.
   Qed.
 
-  Lemma istep_ITV α αv β σ σ' :
-    (IT_to_V α ≡ Some αv ⊢ istep α σ β σ' -∗ False : iProp)%I.
+  Lemma internal_step_ITV α αv β σ σ' en :
+    (IT_to_V α ≡ Some αv ⊢ internal_step α σ β σ' en -∗ False : iProp)%I.
   Proof.
-    rewrite /istep/=. iIntros "Hv [[H _]|H]".
+    rewrite /internal_step/=. iIntros "Hv [[H _]|H]".
     - iRewrite "H" in "Hv". rewrite IT_to_V_Tau.
       iApply (option_equivI with "Hv").
     - iDestruct "H" as (op i k) "[H _]".
@@ -278,23 +581,26 @@ Section istep.
       iApply (option_equivI with "Hv").
   Qed.
 
-  Lemma istep_err σ e β σ' : istep (Err e) σ β σ' ⊢ False.
+  Lemma internal_step_err σ e β σ' en : internal_step (Err e) σ β σ' en ⊢ False.
   Proof.
-    rewrite /istep/=. iDestruct 1 as "[[H _]|H]".
+    rewrite /internal_step/=. iDestruct 1 as "[[H _]|H]".
     - iApply (IT_tick_err_ne).
       by iApply (internal_eq_sym with "H").
     - iDestruct "H" as (op i k) "[H _]". iApply (IT_vis_err_ne).
       by iApply internal_eq_sym.
   Qed.
-  Lemma istep_tick α β σ σ' : istep (Tick α) σ β σ' ⊢ ▷ (β ≡ α) ∧ σ ≡ σ'.
+
+  Lemma internal_step_tick α β σ σ' en :
+    internal_step (Tick α) σ β σ' en ⊢ ▷ (β ≡ α) ∧ σ ≡ σ' ∧ en ≡ [].
   Proof.
-    simpl. iDestruct 1 as "[[H1 H2]|H]".
+    simpl. iDestruct 1 as "[[H1 [H2 H3]]|H]".
     - iFrame. iNext. by iApply internal_eq_sym.
     - iDestruct "H" as (op i k) "[H1 H2]".
       iExFalso. iApply (IT_tick_vis_ne with "H1").
   Qed.
-  Lemma istep_vis op i ko β σ σ' :
-    istep (Vis op i ko) σ β σ' ⊢ reify r (Vis op i ko) σ ≡ (σ', Tick β).
+
+  Lemma internal_step_vis op i ko β σ σ' en :
+    internal_step (Vis op i ko) σ β σ' en ⊢ reify r (Vis op i ko) σ ≡ (σ', Tick β, en).
   Proof.
     simpl. iDestruct 1 as "[[H1 H2]|H]".
     - iExFalso. iApply IT_tick_vis_ne.
@@ -302,15 +608,15 @@ Section istep.
     - iDestruct "H" as (op' i' ko') "[H1 $]".
   Qed.
 
-  Lemma isteps_val βv β k σ σ' :
-    isteps (IT_of_V βv) σ β σ' k ⊢ IT_of_V βv ≡ β ∧ σ ≡ σ' ∧ ⌜k = 0⌝.
+  Lemma internal_steps_val βv β en k σ σ' :
+    internal_steps (IT_of_V βv) σ β σ' en k ⊢ IT_of_V βv ≡ β ∧ σ ≡ σ' ∧ ⌜k = 0⌝ ∧ en ≡ [].
   Proof.
     destruct k as[|k].
-    - rewrite isteps_0. iDestruct 1 as "[$ $]".
+    - rewrite internal_steps_0. iDestruct 1 as "[$ [$ $]]".
       eauto.
-    - rewrite isteps_S. iDestruct 1 as (α1 σ1) "[Hs Hss]".
+    - rewrite internal_steps_S. iDestruct 1 as (α1 σ1 l' l'') "[Heq [Hs Hss]]".
       iExFalso. iClear "Hss".
-      unfold istep. simpl. iDestruct "Hs" as "[[Ht Hs]|Hs]".
+      unfold internal_step. simpl. iDestruct "Hs" as "[[Ht Hs]|Hs]".
       + destruct βv as[n|f]; iSimpl in "Ht".
         ++  iApply (IT_ret_tick_ne with "Ht").
         ++  iApply (IT_fun_tick_ne with "Ht").
@@ -319,27 +625,31 @@ Section istep.
         ++  iApply (IT_ret_vis_ne with "Ht").
         ++  iApply (IT_fun_vis_ne with "Ht").
   Qed.
-  Lemma isteps_tick α βv σ σ' k :
-    isteps (Tick α) σ (IT_of_V βv) σ' k
-    ⊢ ∃ k' : nat, ⌜k = (1 + k')%nat⌝ ∧ ▷ isteps α σ (IT_of_V βv) σ' k'.
+
+  Lemma internal_steps_tick α βv σ σ' l k :
+    internal_steps (Tick α) σ (IT_of_V βv) σ' l k
+    ⊢ ∃ k' : nat, ⌜k = (1 + k')%nat⌝ ∧ ▷ internal_steps α σ (IT_of_V βv) σ' l k'.
   Proof.
-    rewrite isteps_unfold.
+    rewrite internal_steps_unfold.
     iDestruct 1 as "[[Hk [Ht Hs]] | H]".
     - iExFalso. destruct βv; iSimpl in "Ht".
       ++ iApply (IT_ret_tick_ne).
          iApply (internal_eq_sym with "Ht").
       ++ iApply (IT_fun_tick_ne).
          by iApply (internal_eq_sym with "Ht").
-    - iDestruct "H" as (k' α1 σ1) "[% [Hs Hss]]".
+    - iDestruct "H" as (k' α1 σ1 l' l'') "[Hl [% [Hs Hss]]]".
       iExists k'. iSplit; first by eauto.
-      rewrite istep_tick.
-      iDestruct "Hs" as "[Ha Hs]". iNext.
-      iRewrite -"Ha". iRewrite "Hs". done.
+      rewrite internal_step_tick.
+      iDestruct "Hs" as "[Ha [Hs1 Hs2]]". iNext.
+      iRewrite -"Ha". iRewrite "Hs1".
+      iRewrite "Hl".
+      iRewrite "Hs2".
+      done.
   Qed.
 
-End istep.
+End internal_step.
 
-Section istep_ctx_indep.
+Section internal_step_ctx_indep.
   Context {A} `{!Cofe A}.
   Context (r : sReifier NotCtxDep).
   Notation F := (sReifier_ops r).
@@ -351,8 +661,8 @@ Section istep_ctx_indep.
   Context `{!invGS_gen hlc Σ}.
   Notation iProp := (iProp Σ).
 
-  Lemma istep_hom (f : IT → IT) `{!IT_hom f} α σ β σ' :
-    istep r α σ β σ' ⊢ istep r (f α) σ (f β) σ' : iProp.
+  Lemma internal_step_hom (f : IT → IT) `{!IT_hom f} α σ β σ' en :
+    internal_step r α σ β σ' en ⊢ internal_step r (f α) σ (f β) σ' en : iProp.
   Proof.
     iDestruct 1 as "[[Ha Hs]|H]".
     - iRewrite "Ha". iLeft. iSplit; eauto. iPureIntro. apply hom_tick.
@@ -366,15 +676,15 @@ Section istep_ctx_indep.
       iApply (reify_vis_cont with "Hr").
   Qed.
 
-  Lemma istep_hom_inv α σ β σ' (f : IT → IT) `{!IT_hom f} :
-    istep r (f α) σ β σ' ⊢@{iProp} ⌜is_Some (IT_to_V α)⌝
-                          ∨ (IT_to_V α ≡ None ∧ ∃ α', istep r α σ α' σ'
+  Lemma internal_step_hom_inv α σ β σ' en (f : IT → IT) `{!IT_hom f} :
+    internal_step r (f α) σ β σ' en ⊢@{iProp} ⌜is_Some (IT_to_V α)⌝
+                          ∨ (IT_to_V α ≡ None ∧ ∃ α', internal_step r α σ α' σ' en
                                                       ∧ ▷ (β ≡ f α')).
   Proof.
     iIntros "H".
     destruct (IT_dont_confuse α)
       as [[e Ha] | [[n Ha] | [ [g Ha] | [[la Ha]|[op [i [k Ha]]]] ]]].
-    - iExFalso. iApply (istep_err r σ e β σ').
+    - iExFalso. iApply (internal_step_err r σ e β σ').
       iAssert (f α ≡ Err e)%I as "Hf".
       { iPureIntro. by rewrite Ha hom_err. }
       iRewrite "Hf" in "H". done.
@@ -384,17 +694,17 @@ Section istep_ctx_indep.
       iAssert (f (Tick la) ≡ Tick (f la))%I as "Hf".
       { iPureIntro. rewrite hom_tick. done. }
       iRight. iRewrite "Ha". iRewrite "Ha" in "H".
-      iRewrite "Hf" in "H". rewrite istep_tick.
+      iRewrite "Hf" in "H". rewrite internal_step_tick.
       iDestruct "H" as "[Hb Hs]". iSplit.
       { by rewrite IT_to_V_Tau. }
       iExists la. iSplit; last eauto.
-      unfold istep. iLeft. iSplit; eauto.
+      unfold internal_step. iLeft. iSplit; eauto.
     - iRight.
       pose (fi:=OfeMor f).
       iAssert (f α ≡ Vis op i (laterO_map fi ◎ k))%I as "Hf".
       { iPureIntro. by rewrite Ha hom_vis. }
       iRewrite "Hf" in "H".
-      rewrite {1}/istep. iSimpl in "H".
+      rewrite {1}/internal_step. iSimpl in "H".
       iDestruct "H" as "[[H _]|H]".
       + iExFalso. iApply (IT_tick_vis_ne).
         iApply internal_eq_sym. done.
@@ -402,13 +712,13 @@ Section istep_ctx_indep.
         iPoseProof (Vis_inj_op' with "Ha") as "<-".
         iPoseProof (Vis_inj' with "Ha") as "[Hi Hk]".
         iPoseProof (reify_input_cont_inv r op i k fi with "Hr") as (α') "[Hr Ha']".
-        iAssert (reify r α σ ≡ (σ', Tick α'))%I with "[Hr]" as "Hr".
+        iAssert (reify r α σ ≡ (σ', Tick α', en))%I with "[Hr]" as "Hr".
         { iRewrite -"Hr". iPureIntro. repeat f_equiv.
           apply Ha. }
         iSplit. { iPureIntro. by rewrite Ha IT_to_V_Vis. }
         iExists α'. iFrame "Ha'".
-        rewrite /istep. iRight.
+        rewrite /internal_step. iRight.
         iExists op,i,k. iFrame "Hr".
         iPureIntro. apply Ha.
   Qed.
-End istep_ctx_indep.
+End internal_step_ctx_indep.
