theories/effects/delim.v
@@ -74,48 +74,46 @@ Section reifiers.
 
   Definition reify_shift : ((laterO X -n> laterO X) -n> laterO X) *
                               state * (laterO X -n> laterO X) →
-                            option (laterO X * state) :=
-    λ '(f, σ, k), Some ((f k): laterO X, σ : state).
+                            option (laterO X * state * listO (laterO X)) :=
+    λ '(f, σ, k), Some ((f k): laterO X, σ : state, []).
   #[export] Instance reify_shift_ne :
     NonExpansive (reify_shift :
       prodO (prodO ((laterO X -n> laterO X) -n> laterO X) state)
         (laterO X -n> laterO X) →
-      optionO (prodO (laterO X) state)).
+      optionO ((laterO X) * state * listO (laterO X))%type).
   Proof. intros ?[[]][[]][[]]. simpl in *. repeat f_equiv; auto. Qed.
 
   Definition reify_reset : (laterO X) * state * (laterO X -n> laterO X) →
-                           option (laterO X * state) :=
-    λ '(e, σ, k), Some (e, (k :: σ)).
+                           option (laterO X * state * listO (laterO X)) :=
+    λ '(e, σ, k), Some (e, (k :: σ), []).
   #[export] Instance reify_reset_ne :
     NonExpansive (reify_reset :
         prodO (prodO (laterO X) state) (laterO X -n> laterO X) →
-        optionO (prodO (laterO X) state)).
+        optionO ((laterO X) * state * listO (laterO X))%type).
   Proof. intros ?[[]][[]][[]]. simpl in *. by repeat f_equiv. Qed.
 
-
   Definition reify_pop : (laterO X) * state * (Empty_setO -n> laterO X) →
-                           option (laterO X * state) :=
+                           option (laterO X * state * listO (laterO X)) :=
     λ '(e, σ, _),
       match σ with
-      | [] => Some (e, σ)
-      | k' :: σ' => Some (k' e, σ')
+      | [] => Some (e, σ, [])
+      | k' :: σ' => Some (k' e, σ', [])
       end.
   #[export] Instance reify_pop_ne :
     NonExpansive (reify_pop :
         prodO (prodO (laterO X) state) (Empty_setO -n> laterO X) →
-        optionO (prodO (laterO X) state)).
+        optionO ((laterO X) * state * listO (laterO X))%type).
   Proof. intros ?[[]][[]][[]]. simpl in *. by repeat f_equiv. Qed.
 
-
   Definition reify_app_cont : ((laterO X * (laterO (X -n> X))) * state * (laterO X -n> laterO X)) →
-                              option (laterO X * state) :=
+                              option (laterO X * state * listO (laterO X)) :=
   λ '((e, k'), σ, k),
-    Some (((laterO_ap k' : laterO X -n> laterO X) e : laterO X), k::σ : state).
+    Some (((laterO_ap k' : laterO X -n> laterO X) e : laterO X), k::σ : state, []).
   #[export] Instance reify_app_cont_ne :
     NonExpansive (reify_app_cont :
         prodO (prodO (prodO (laterO X) (laterO (X -n> X))) state)
           (laterO X -n> laterO X) →
-        optionO (prodO (laterO X) (state))).
+        optionO ((laterO X) * (state) * listO (laterO X))%type).
   Proof.
     intros ?[[[]]][[[]]]?. rewrite /reify_app_cont.
     repeat f_equiv; apply H.
@@ -239,12 +237,17 @@ Section weakestpre.
     rewrite hom_vis.
     iApply (wp_subreify_ctx_dep _ _ _ _ _ _ _ (laterO_map 𝒫 $ f (laterO_map k)) with "Hs").
     {
-      simpl. do 2 f_equiv; last done. do 2 f_equiv.
+      simpl. do 2 f_equiv; last done.
+      f_equiv; last done.
+      do 2 f_equiv.
       rewrite ccompose_id_l. intro. simpl. by rewrite ofe_iso_21.
     }
     { exact Hp. }
-    iModIntro.
-    iApply "Ha".
+    rewrite /=.
+    iNext.
+    iIntros "Hlc Hs".
+    iSplit; last done.
+    iApply ("Ha" with "Hlc Hs").
   Qed.
 
   Lemma wp_reset (σ : state) (e : IT) (k : IT -n> IT) {Hk : IT_hom k}
@@ -257,11 +260,15 @@ Section weakestpre.
     iIntros "Hs Ha".
     unfold RESET. simpl. rewrite hom_vis.
     iApply (wp_subreify_ctx_dep _ _ _ _ _ _ _ (Next $ 𝒫 e) with "Hs").
-    - simpl. repeat f_equiv. rewrite ccompose_id_l.
-      trans ((laterO_map k) :: σ); last reflexivity.
-      f_equiv. intro. simpl. by rewrite ofe_iso_21.
+    - simpl. f_equiv. rewrite ccompose_id_l later_map_Next.
+      trans (Next (𝒫 e), (laterO_map k) :: σ, [] : listO (laterO IT)); last reflexivity.
+      do 3 f_equiv. intro. simpl. by rewrite ofe_iso_21.
     - reflexivity.
-    - iApply "Ha".
+    - rewrite /=.
+      iNext.
+      iIntros "Hlc Hs".
+      iSplit; last done.
+      iApply ("Ha" with "Hlc Hs").
   Qed.
 
   Lemma wp_pop_end (v : IT)
@@ -276,7 +283,11 @@ Section weakestpre.
     iApply (wp_subreify_ctx_dep _ _ _ _ _ _ _ ((Next v)) with "Hs").
     - simpl. reflexivity.
     - reflexivity.
-    - done.
+    - rewrite /=.
+      iNext.
+      iIntros "Hlc Hs".
+      iSplit; last done.
+      iApply ("Ha" with "Hlc Hs").
   Qed.
 
   Lemma wp_pop_cons (σ : state) (v : IT) (k : IT -n> IT)
@@ -291,147 +302,12 @@ Section weakestpre.
     iApply (wp_subreify_ctx_dep _ _ _ _ _ _ _ ((laterO_map k (Next v))) with "Hs").
     - simpl. reflexivity.
     - reflexivity.
-    - done.
+    - rewrite /=.
+      iNext.
+      iIntros "Hlc Hs".
+      iSplit; last done.
+      iApply ("Ha" with "Hlc Hs").
   Qed.
-
-  (* Lemma wp_get_val (α : IT) (f : IT -n> IT) *)
-  (*   Φ `{!NonExpansive Φ} s : *)
-  (*   WP@{rs} α @ s {{ βv, WP@{rs} (f (IT_of_V βv)) @ s {{ Φ }} }} *)
-  (*   -∗ WP@{rs} get_val f α @ s {{ Φ }}. *)
-  (* Proof. *)
-  (*   iLöb as "IH" forall ( α ). *)
-  (*   iIntros "Ha". *)
-  (*   destruct (IT_dont_confuse α) *)
-  (*     as [[e ->] | [[m ->] | [ [g ->] | [[α' ->]|[op [i [ko ->]]]] ]]]. *)
-  (*   - rewrite get_val_err. *)
-  (*     rewrite ->wp_unfold at 1. *)
-  (*     iDestruct "Ha" as "[Ha | Ha]". *)
-  (*     + iDestruct "Ha" as "(%αv & Ha & _)". *)
-  (*       rewrite IT_to_V_Err. *)
-  (*       by iPoseProof (option_equivI with "Ha") as "Ha". *)
-  (*     + iDestruct "Ha" as "(H1 & H2)". *)
-  (*       iEval (rewrite wp_unfold). *)
-  (*       iRight. *)
-  (*       iSplit; first done. *)
-  (*       iIntros (σ) "Hσ". *)
-  (*       iSpecialize ("H2" $! σ with "Hσ"). *)
-  (*       iMod "H2". *)
-  (*       iDestruct "H2" as "(H2 & H3)". *)
-  (*       iDestruct "H2" as "[H2 | H2]". *)
-  (*       * iDestruct "H2" as "(%α' & %σ' & H2)". *)
-  (*         iExFalso. *)
-  (*         by iDestruct (istep_err with "H2") as "H2". *)
-  (*       * iDestruct "H2" as "(%err & HEQ & H2)". *)
-  (*         iDestruct (Err_inj' with "HEQ") as "%HEQ". *)
-  (*         rewrite HEQ. *)
-  (*         iModIntro. *)
-  (*         iSplit. *)
-  (*         -- iRight. *)
-  (*            iExists err. *)
-  (*            iSplit; done. *)
-  (*         -- iIntros (σ' β) "Hst Hc". *)
-  (*            iExFalso. *)
-  (*            iDestruct "Hst" as "[(Hst & _) | (%op & %i & %k & Hst & _)]". *)
-  (*            ++ iDestruct (internal_eq_sym with "Hst") as "Hst". *)
-  (*               by iDestruct (IT_tau_err_ne with "Hst") as "Hst". *)
-  (*            ++ iDestruct (internal_eq_sym with "Hst") as "Hst". *)
-  (*               by iDestruct (IT_vis_err_ne with "Hst") as "Hst". *)
-  (*   - rewrite core.get_val_ret. *)
-  (*     iDestruct (wp_val_inv with "Ha") as "Ha"; *)
-  (*       first solve_proper. *)
-  (*     by iApply fupd_wp. *)
-  (*   - rewrite get_val_fun. *)
-  (*     iDestruct (wp_val_inv with "Ha") as "Ha"; *)
-  (*       first solve_proper. *)
-  (*     by iApply fupd_wp. *)
-  (*   - rewrite get_val_tick. *)
-  (*     rewrite ->wp_unfold at 1. *)
-  (*     iDestruct "Ha" as "[Ha | Ha]". *)
-  (*     + iDestruct "Ha" as "(%αv & Ha & _)". *)
-  (*       rewrite IT_to_V_Tick. *)
-  (*       by iPoseProof (option_equivI with "Ha") as "Ha". *)
-  (*     + iDestruct "Ha" as "(H1 & H2)". *)
-  (*       iEval (rewrite wp_unfold). *)
-  (*       iRight. *)
-  (*       iSplit. *)
-  (*       { *)
-  (*         iClear "∗". rewrite IT_to_V_Tick. *)
-  (*         done. *)
-  (*       } *)
-  (*       iIntros (σ) "Hσ". *)
-  (*       iSpecialize ("H2" $! σ with "Hσ"). *)
-  (*       iMod "H2". *)
-  (*       iDestruct "H2" as "(H2 & H3)". *)
-  (*       iDestruct "H2" as "[H2 | H2]". *)
-  (*       * iDestruct "H2" as "(%α'' & %σ' & #H2)". *)
-  (*         iSpecialize ("H3" $! σ' α'' with "H2"). *)
-  (*         iModIntro. *)
-  (*         iSplit. *)
-  (*         -- iLeft. *)
-  (*            iExists (get_val f α'). *)
-  (*            iExists σ. *)
-  (*            iLeft. *)
-  (*            iSplit; done. *)
-  (*         -- iIntros (σ'' α''') "#H4 Hc". *)
-  (*            iSpecialize ("H3" with "Hc"). *)
-  (*            iMod "H3". *)
-  (*            iModIntro. *)
-  (*            iNext. *)
-  (*            iMod "H3". *)
-  (*            iModIntro. *)
-  (*            iMod "H3". *)
-  (*            iModIntro. *)
-  (*            iDestruct "H4" as "[H4 | H4]". *)
-  (*            ++ iDestruct "H4" as "(HEQ1 & HEQ2)". *)
-  (*               iRewrite -"HEQ1". *)
-  (*               iRewrite -"HEQ2". *)
-  (*               iClear "HEQ1 HEQ2". *)
-  (*               iDestruct "H2" as "[H2 | H2]". *)
-  (*               ** iDestruct "H2" as "(HEQ1 & HEQ2)". *)
-  (*                  iRewrite "HEQ1". *)
-  (*                  iRewrite "HEQ2". *)
-  (*                  iClear "HEQ1 HEQ2". *)
-  (*                  iDestruct "H3" as "($ & H3)". *)
-  (*                  by iApply "IH". *)
-  (*               ** iDestruct "H2" as "(%op & %i & %k & Hst & _)". *)
-  (*                  iExFalso. *)
-  (*                  by iDestruct (IT_tau_vis_ne with "Hst") as "Hst'". *)
-  (*            ++ iDestruct "H4" as "(%op & %i & %k & Hst & _)". *)
-  (*               iExFalso. *)
-  (*               by iDestruct (IT_tau_vis_ne with "Hst") as "Hst'". *)
-  (*       * iDestruct "H2" as "(%err & HEQ & H2)". *)
-  (*         by iDestruct (IT_tau_err_ne with "HEQ") as "HEQ". *)
-  (*   - rewrite get_val_vis. *)
-  (*     iClear "IH". *)
-  (*     rewrite ->wp_unfold at 1. *)
-  (*     iDestruct "Ha" as "[Ha | Ha]". *)
-  (*     + iDestruct "Ha" as "(%αv & Ha & _)". *)
-  (*       rewrite IT_to_V_Vis. *)
-  (*       by iPoseProof (option_equivI with "Ha") as "Ha". *)
-  (*     + iDestruct "Ha" as "(H1 & H2)". *)
-  (*       iEval (rewrite wp_unfold). *)
-  (*       iRight. *)
-  (*       iSplit. *)
-  (*       { *)
-  (*         iClear "∗". rewrite IT_to_V_Vis. *)
-  (*         done. *)
-  (*       } *)
-  (*       iIntros (σ) "Hσ". *)
-  (*       iSpecialize ("H2" $! σ with "Hσ"). *)
-  (*       iMod "H2". *)
-  (*       iDestruct "H2" as "(H2 & H3)". *)
-  (*       iDestruct "H2" as "[H2 | H2]". *)
-  (*       * iDestruct "H2" as "(%α'' & %σ' & #H2)". *)
-  (*         iModIntro. *)
-  (*         iSplit. *)
-  (*         -- iLeft. *)
-  (*            admit. *)
-  (*         -- iIntros (σ'' β) "Hst Hc". *)
-  (*            iSpecialize ("H3" $! σ' β). *)
-  (*            admit. *)
-  (*       * iDestruct "H2" as "(%err & HEQ & H2)". *)
-  (*         by iDestruct (IT_vis_err_ne with "HEQ") as "HEQ". *)
-  (* Admitted.         *)
 
   Lemma wp_app_cont (σ : state) (e : laterO IT) (k' : laterO (IT -n> IT))
     (k : IT -n> IT) β {Hk : IT_hom k}
@@ -445,11 +321,16 @@ Section weakestpre.
     iIntros (Hb) "Hs Ha".
     unfold APP_CONT. simpl. rewrite hom_vis.
     iApply (wp_subreify_ctx_dep _ _ _ _ _ _ _ (Next β) with "Hs").
-    - cbn-[laterO_ap]. rewrite Hb. do 2 f_equiv.
-      trans (laterO_map k :: σ); last reflexivity.
+    - cbn-[laterO_ap]. rewrite Hb.
+      trans (Some (Next β, laterO_map k :: σ, [] : listO (laterO IT))); last reflexivity.
+      do 3 f_equiv.
       rewrite ccompose_id_l. f_equiv. intro. simpl. by rewrite ofe_iso_21.
     - reflexivity.
-    - iApply "Ha".
+    - rewrite /=.
+      iNext.
+      iIntros "Hlc Hs".
+      iSplit; last done.
+      iApply ("Ha" with "Hlc Hs").
   Qed.
 
 End weakestpre.
