theories/effects/fork.v
@@ -1,0 +1,92 @@
+From gitrees Require Import prelude gitree.
+Require Import iris.algebra.list.
+
+Definition state := unitO.
+#[export] Instance state_inhabited : Inhabited state := populate ().
+
+Notation stateO := (leibnizO state).
+
+Program Definition forkI : opInterp :=
+  {|
+    Ins := (▶ ∙);
+    Outs := unitO;
+  |}.
+
+Definition concE := @[forkI].
+
+(* FORK *)
+Definition reify_fork X `{Cofe X} : (laterO X) * stateO →
+                                      option (unitO * stateO * listO (laterO X)) :=
+    λ '(o, σ), Some ((), σ, [o]).
+#[export] Instance reify_fork_ne X `{Cofe X} :
+  NonExpansive (reify_fork X).
+Proof.
+  intros ?[? []] [? []] G.
+  simpl in *. f_equiv.
+  do 2 f_equiv.
+  apply G.
+Qed.
+
+Canonical Structure reify_fork_sig : sReifier NotCtxDep.
+Proof.
+  simple refine {| sReifier_ops := concE;
+                   sReifier_state := stateO
+                |}.
+  intros X HX op.
+  destruct op as [? | []]; simpl.
+  simple refine (OfeMor (reify_fork X)).
+Defined.
+
+Section constructors.
+  Context {E : opsInterp} {A} `{!Cofe A}.
+  Context {subEff0 : subEff concE E}.
+  Context {subOfe0 : SubOfe unitO A}.
+  Notation IT := (IT E A).
+  Notation ITV := (ITV E A).
+
+  Program Definition FORK : IT -n> IT :=
+    λne k, Vis (E:=E) (subEff_opid (inl ()))
+             (subEff_ins (F:=concE) (op:=(inl ())) (Next k))
+             (NextO ◎ Ret ◎ (subEff_outs (F:=concE) (op:=(inl ())))^-1).
+  Solve Obligations with solve_proper.
+End constructors.
+
+Section weakestpre.
+  Context {sz : nat}.
+  Context {a : is_ctx_dep}.
+  Variable (rs : gReifiers a sz).
+  Context {subR : subReifier (sReifier_NotCtxDep_min reify_fork_sig a) rs}.
+  Notation F := (gReifiers_ops rs).
+  Context {R} `{!Cofe R}.
+  Context `{!SubOfe unitO R}.
+  Notation IT := (IT F R).
+  Notation ITV := (ITV F R).
+  Context `{!invGS Σ, !stateG rs R Σ}.
+  Notation iProp := (iProp Σ).
+
+  Lemma wp_fork (σ : stateO) (n : IT) (k : IT -n> IT) `{!IT_hom k} Φ s :
+    has_substate σ
+    -∗ ▷ (£ 1 -∗ has_substate σ -∗ WP@{rs} (k (Ret ())) @ s {{ Φ }}
+                                 ∗ ▷ WP@{rs} n @ s {{ constO True }}) -∗
+    WP@{rs} k (FORK n) @ s {{ Φ }}.
+  Proof.
+    iIntros "Hs Ha".
+    unfold FORK. simpl.
+    rewrite hom_vis.
+    iApply wp_subreify_ctx_indep_lift''.
+    iModIntro.
+    iExists σ, (), σ, (k (Ret ())), [NextO n].
+    iFrame "Hs".
+    iSplit; first done.
+    rewrite /= ofe_iso_21 later_map_Next.
+    iSplit; first done.
+    iNext.
+    iIntros "Hc Hs !>".
+    iDestruct ("Ha" with "Hc Hs") as "(Ha1 & Ha2)".
+    iSplitL "Ha1"; first done.
+    rewrite -Tick_eq.
+    iSplit; last done.
+    by iApply wp_tick.
+  Qed.
+
+End weakestpre.
