theories/gitree/greifiers.v
@@ -1,3 +1,4 @@
+From iris.algebra Require Import list.
 From iris.proofmode Require Import classes tactics.
 From iris.base_logic.lib Require Export invariants.
 From gitrees Require Import prelude.
@@ -123,7 +124,7 @@ Section greifiers.
   Program Definition gReifiers_re_ctx_indep {n} (rs : gReifiers NotCtxDep n) {X} `{!Cofe X}
     (op : opid (gReifiers_ops NotCtxDep rs)) :
     (Ins (gReifiers_ops NotCtxDep rs op) ♯ X) * (gReifiers_state NotCtxDep rs ♯ X) -n>
-      optionO ((Outs (gReifiers_ops NotCtxDep rs op) ♯ X) * (gReifiers_state NotCtxDep rs ♯ X))
+      optionO ((Outs (gReifiers_ops NotCtxDep rs op) ♯ X) * (gReifiers_state NotCtxDep rs ♯ X) * listO (laterO X))
     :=  λne xst,
       let  i := projT1 op in
       let op' := projT2 op in
@@ -133,14 +134,14 @@ Section greifiers.
       let σ := fs.1 in
       let rest := fs.2 in
       let rx := sReifier_re (rs !!! i) op' (x, σ) in
-      optionO_map (prodO_map idfun (gState_recomp NotCtxDep rest)) rx.
+      optionO_map (prodO_map (prodO_map idfun (gState_recomp NotCtxDep rest)) idfun) rx.
   Next Obligation. solve_proper_please. Qed.
 
   Program Definition gReifiers_re_ctx_dep {n} (rs : gReifiers CtxDep n) {X} `{!Cofe X}
     (op : opid (gReifiers_ops CtxDep rs)) :
     (Ins (gReifiers_ops CtxDep rs op) ♯ X) * (gReifiers_state CtxDep rs ♯ X)
     * ((Outs (gReifiers_ops CtxDep rs op) ♯ X) -n> laterO X) -n>
-      optionO (laterO X * (gReifiers_state CtxDep rs ♯ X))
+      optionO (laterO X * (gReifiers_state CtxDep rs ♯ X) * listO (laterO X))
     :=  λne xst,
       let  i := projT1 op in
       let op' := projT2 op in
@@ -151,7 +152,7 @@ Section greifiers.
       let σ := fs.1 in
       let rest := fs.2 in
       let rx := sReifier_re (rs !!! i) op' (a, σ, c) in
-      optionO_map (prodO_map idfun (gState_recomp CtxDep rest)) rx.
+      optionO_map (prodO_map (prodO_map idfun (gState_recomp CtxDep rest)) idfun) rx.
   Next Obligation. solve_proper_please. Qed.
 
   Program Definition gReifiers_re_type {n}
@@ -161,10 +162,10 @@ Section greifiers.
     | CtxDep =>
         prodO (prodO (Ins (gReifiers_ops a rs op) ♯ X) (gReifiers_state a rs ♯ X))
           (Outs (gReifiers_ops a rs op) ♯ X -n> laterO X) -n>
-          optionO (prodO (laterO X) (gReifiers_state a rs ♯ X))
+          optionO (prodO (prodO (laterO X) (gReifiers_state a rs ♯ X)) (listO (laterO X)))
     | NotCtxDep =>
         prodO (Ins (gReifiers_ops a rs op) ♯ X) (gReifiers_state a rs ♯ X) -n>
-          optionO (prodO (Outs (gReifiers_ops a rs op) ♯ X) (gReifiers_state a rs ♯ X))
+          optionO (prodO (prodO (Outs (gReifiers_ops a rs op) ♯ X) (gReifiers_state a rs ♯ X)) (listO (laterO X)))
     end.
 
   Program Definition gReifiers_re {n} (a : is_ctx_dep) (rs : gReifiers a n)
@@ -186,7 +187,9 @@ Section greifiers.
     |}.
   Next Obligation.
     intros n [|] rs X ? op.
-    - apply (@gReifiers_re n CtxDep rs X _ op).
+    - pose proof (@gReifiers_re n CtxDep rs X _ op).
+      simpl in *.
+      apply (@gReifiers_re n CtxDep rs X _ op).
     - apply (@gReifiers_re n NotCtxDep rs X _ op).
   Defined.
 
@@ -197,14 +200,13 @@ Section greifiers.
     (rest : gState_rest CtxDep i rs ♯ X)
     (κ : (Outs (sReifier_ops (rs !!! i) op) ♯ X -n> laterO X)) :
     gReifiers_re CtxDep rs (existT i op) (x, gState_recomp CtxDep rest σ, κ) ≡
-      optionO_map (prodO_map idfun (gState_recomp CtxDep rest))
+      optionO_map (prodO_map (prodO_map idfun (gState_recomp CtxDep rest)) idfun)
       (sReifier_re (rs !!! i) op (x, σ, κ)).
   Proof.
     unfold gReifiers_re. cbn-[prodO_map optionO_map].
     f_equiv; last repeat f_equiv.
     - eapply optionO_map_proper.
-      intros [x1 x2]; simpl. f_equiv.
-      f_equiv. f_equiv.
+      intros [[x1 x3] x2]; simpl. do 2 f_equiv.
       rewrite gState_decomp_recomp//.
     - rewrite gState_decomp_recomp//.
   Qed.
@@ -215,13 +217,13 @@ Section greifiers.
     (σ : sReifier_state (rs !!! i) ♯ X)
     (rest : gState_rest NotCtxDep i rs ♯ X) :
     gReifiers_re NotCtxDep rs (existT i op) (x, gState_recomp NotCtxDep rest σ) ≡
-      optionO_map (prodO_map idfun (gState_recomp NotCtxDep rest))
+      optionO_map (prodO_map (prodO_map idfun (gState_recomp NotCtxDep rest)) idfun)
       (sReifier_re (rs !!! i) op (x, σ)).
   Proof.
     unfold gReifiers_re. cbn-[prodO_map optionO_map].
     f_equiv; last repeat f_equiv.
     - eapply optionO_map_proper.
-      intros [x1 x2]; simpl. f_equiv.
+      intros [[x1 x3] x2]; simpl. do 2 f_equiv.
       f_equiv. f_equiv.
       rewrite gState_decomp_recomp//.
     - rewrite gState_decomp_recomp//.
@@ -237,10 +239,10 @@ Section greifiers.
     destruct a.
     - apply (∀ (κ : (Outs (sReifier_ops (rs !!! i) op) ♯ X -n> laterO X)),
                gReifiers_re CtxDep rs (existT i op) (x, gState_recomp CtxDep rest σ, κ) ≡
-                 optionO_map (prodO_map idfun (gState_recomp CtxDep rest))
+                 optionO_map (prodO_map (prodO_map idfun (gState_recomp CtxDep rest)) idfun)
                  (sReifier_re (rs !!! i) op (x, σ, κ))).
     - apply (gReifiers_re NotCtxDep rs (existT i op) (x, gState_recomp NotCtxDep rest σ) ≡
-               optionO_map (prodO_map idfun (gState_recomp NotCtxDep rest))
+               optionO_map (prodO_map (prodO_map idfun (gState_recomp NotCtxDep rest)) idfun)
                (sReifier_re (rs !!! i) op (x, σ))).
   Defined.
 
@@ -266,18 +268,18 @@ Section greifiers.
     - apply (∀ (x : Ins (sReifier_ops r op) ♯ X)
                (y : laterO X)
                (s1 s2 : sReifier_state r ♯ X)
-               (k : (Outs (sReifier_ops r op) ♯ X -n> laterO X)),
-               sReifier_re r op (x, s1, k) ≡{m}≡ Some (y, s2) →
+               (k : (Outs (sReifier_ops r op) ♯ X -n> laterO X)) th,
+               sReifier_re r op (x, s1, k) ≡{m}≡ Some (y, s2, th) →
                @sReifier_re CtxDep (rs !!! sR_idx) _ _ (subEff_opid op)
                  (subEff_ins x, sR_state s1, k ◎ (subEff_outs ^-1)) ≡{m}≡
-                 Some (y, sR_state s2)).
+                 Some (y, sR_state s2, th)).
     - apply (∀ (x : Ins (sReifier_ops _ op) ♯ X)
                (y : Outs (sReifier_ops _ op) ♯ X)
-               (s1 s2 : sReifier_state r ♯ X),
-               sReifier_re r op (x, s1) ≡{m}≡ Some (y, s2) →
+               (s1 s2 : sReifier_state r ♯ X) th,
+               sReifier_re r op (x, s1) ≡{m}≡ Some (y, s2, th) →
                @sReifier_re NotCtxDep (rs !!! sR_idx) _ _ (subEff_opid op)
                  (subEff_ins x, sR_state s1) ≡{m}≡
-                 Some (subEff_outs y, sR_state s2)).
+                 Some (subEff_outs y, sR_state s2, th)).
   Defined.
 
   Class subReifier {n} {a : is_ctx_dep} (r : sReifier a) (rs : gReifiers a n) :=
@@ -297,11 +299,11 @@ Section greifiers.
     - simpl. apply subEff_id.
     - simpl. intros. apply iso_ofe_refl.
     - destruct a.
-      + intros X ? op x y ? s1 s2 k HEQ; simpl.
+      + intros X ? op x y ? s1 s2 k th HEQ; simpl.
         unfold ofe_iso_1'; simpl.
         rewrite ccompose_id_r HEQ.
         reflexivity.
-      + intros X ? op x y s1 s2.
+      + intros X ? op x y o s2 s3 th.
         simpl. eauto.
   Defined.
 
@@ -314,12 +316,12 @@ Section greifiers.
     simple refine ({| sR_idx := FS sR_idx |}).
     - simpl. intros. apply sR_state.
     - destruct a.
-      + intros ? X ? op x y s1 s2.
+      + intros ? X ? op x y s1 s2 k th.
         simpl. intros.
         pose proof (@sR_re n CtxDep r rs _ m X _ op) as G.
         simpl in G.
         by apply G.
-      + intros ? X ? op x y s1 s2.
+      + intros ? X ? op x y s1 s2 th.
         simpl. intros.
         pose proof (@sR_re n NotCtxDep r rs _ m X _ op) as G.
         simpl in G.
@@ -365,18 +367,18 @@ Section greifiers.
     - apply (∀ (x : Ins (sReifier_ops r op) ♯ X)
                (y : laterO X)
                (s1 s2 : sReifier_state r ♯ X)
-               (k : (Outs (sReifier_ops r op) ♯ X -n> laterO X)),
-               sReifier_re r op (x, s1, k) ≡ Some (y, s2) →
+               (k : (Outs (sReifier_ops r op) ♯ X -n> laterO X)) th,
+               sReifier_re r op (x, s1, k) ≡ Some (y, s2, th) →
                @sReifier_re CtxDep (rs !!! sR_idx) _ _ (subEff_opid op)
                  (subEff_ins x, sR_state s1, k ◎ (subEff_outs ^-1)) ≡
-                 Some (y, sR_state s2)).
+                 Some (y, sR_state s2, th)).
     - apply (∀ (x : Ins (sReifier_ops _ op) ♯ X)
                (y : Outs (sReifier_ops _ op) ♯ X)
-               (s1 s2 : sReifier_state r ♯ X),
-               sReifier_re r op (x, s1) ≡ Some (y, s2) →
+               (s1 s2 : sReifier_state r ♯ X) th,
+               sReifier_re r op (x, s1) ≡ Some (y, s2, th) →
                @sReifier_re NotCtxDep (rs !!! sR_idx) _ _ (subEff_opid op)
                  (subEff_ins x, sR_state s1) ≡
-                 Some (subEff_outs y, sR_state s2)).
+                 Some (subEff_outs y, sR_state s2, th)).
   Defined.
 
   Lemma subReifier_reify_idx {n} {a : is_ctx_dep}
@@ -404,17 +406,17 @@ Section greifiers.
     destruct a.
     - apply (∀ (x : Ins (sReifier_ops _ op) ♯ X) (y : laterO X)
                (k : (Outs (sReifier_ops r op) ♯ X -n> laterO X))
-               (σ σ' : sReifier_state r ♯ X) (rest : gState_rest CtxDep sR_idx rs ♯ X),
-               sReifier_re r op (x, σ, k) ≡ Some (y, σ') →
+               (σ σ' : sReifier_state r ♯ X) (rest : gState_rest CtxDep sR_idx rs ♯ X) th,
+               sReifier_re r op (x, σ, k) ≡ Some (y, σ', th) →
                gReifiers_re CtxDep rs (subEff_opid op)
                  (subEff_ins x, gState_recomp CtxDep rest (sR_state σ), k ◎ (subEff_outs ^-1))
-                 ≡ Some (y, gState_recomp CtxDep rest (sR_state σ'))).
+                 ≡ Some (y, gState_recomp CtxDep rest (sR_state σ'), th)).
     - apply (∀ (x : Ins (sReifier_ops _ op) ♯ X) (y : Outs (sReifier_ops _ op) ♯ X)
-               (σ σ' : sReifier_state r ♯ X) (rest : gState_rest NotCtxDep sR_idx rs ♯ X),
-               sReifier_re r op (x,σ) ≡ Some (y, σ') →
+               (σ σ' : sReifier_state r ♯ X) (rest : gState_rest NotCtxDep sR_idx rs ♯ X) th,
+               sReifier_re r op (x,σ) ≡ Some (y, σ', th) →
                gReifiers_re NotCtxDep rs (subEff_opid op)
                  (subEff_ins x, gState_recomp NotCtxDep rest (sR_state σ))
-                 ≡ Some (subEff_outs y, gState_recomp NotCtxDep rest (sR_state σ'))).
+                 ≡ Some (subEff_outs y, gState_recomp NotCtxDep rest (sR_state σ'), th)).
   Defined.
 
   Lemma subReifier_reify {n} {a : is_ctx_dep} (r : sReifier a)
@@ -423,39 +425,41 @@ Section greifiers.
   Proof.
     destruct a.
     - simpl.
-      intros x y k σ σ' H Hre.
-      pose proof (@subReifier_reify_idx n CtxDep r rs _ X _ op x y σ σ' k Hre) as J; clear Hre.
+      intros x y k σ σ' H th Hre.
+      pose proof (@subReifier_reify_idx n CtxDep r rs _ X _ op x y σ σ' k th Hre) as J; clear Hre.
       simpl in J.
       pose proof (@gReifiers_re_idx n CtxDep sR_idx rs X _ (subEff_opid op)) as J'.
       simpl in J'.
       rewrite J'; clear J'.
-      transitivity (prod_map (λ x0 : laterO X, x0)
+      transitivity (prod_map (prod_map (λ x0 : laterO X, x0)
                       (λ st : sReifier_state (rs !!! sR_idx) ♯ X,
-                          (gState_decomp' CtxDep sR_idx rs ^-1) (st, H)) <$>
-                      (Some (y, sR_state σ'))).
+                          (gState_decomp' CtxDep sR_idx rs ^-1) (st, H))) idfun <$>
+                      (Some (y, sR_state σ', th))).
       + unfold prod_map.
         rewrite option_fmap_proper; [reflexivity | intros ??? | apply J].
-        do 2 f_equiv; first assumption.
-        do 2 f_equiv; assumption.
+        f_equiv; last (simpl; by f_equiv).
+        f_equiv; first (by do 2 f_equiv).
+        by do 4 f_equiv.
       + simpl; reflexivity.
     - simpl.
-      intros x y σ σ' rest Hre.
-      pose proof (@subReifier_reify_idx n NotCtxDep r rs _ X _ op x y σ σ' Hre)
+      intros x y σ σ' rest th Hre.
+      pose proof (@subReifier_reify_idx n NotCtxDep r rs _ X _ op x y σ σ' th Hre)
         as J; clear Hre.
       simpl in J.
       pose proof (@gReifiers_re_idx n NotCtxDep sR_idx rs X _ (subEff_opid op))
         as J'.
       simpl in J'.
       rewrite J'; clear J'.
-      transitivity (prod_map (λ x0 : Outs (sReifier_ops (rs !!! sR_idx)
+      transitivity (prod_map (prod_map (λ x0 : Outs (sReifier_ops (rs !!! sR_idx)
                                              (subEff_opid op)) ♯ X, x0)
                       (λ st : sReifier_state (rs !!! sR_idx) ♯ X,
-                          (gState_decomp' NotCtxDep sR_idx rs ^-1) (st, rest)) <$>
-                      (Some (subEff_outs y, sR_state σ'))).
+                          (gState_decomp' NotCtxDep sR_idx rs ^-1) (st, rest))) idfun <$>
+                      (Some (subEff_outs y, sR_state σ', th))).
       + unfold prod_map.
         rewrite option_fmap_proper; [reflexivity | intros ??? | apply J].
-        do 2 f_equiv; first assumption.
-        do 2 f_equiv; assumption.
+        f_equiv; last (simpl; by f_equiv).
+        f_equiv; first (by do 2 f_equiv).
+        by do 4 f_equiv.
       + simpl; reflexivity.
   Qed.
 
@@ -466,18 +470,18 @@ Section greifiers.
   Notation sr a rs := (gReifiers_sReifier a rs).
 
   Lemma reify_vis_eqI_ctx_dep (rs : gReifiers CtxDep sz)
-    {A} `{!Cofe A} op i k o σ σ' :
-    (gReifiers_re CtxDep rs op (i, σ, k) ≡ Some (o,σ')
-     ⊢@{iProp} reify (sr CtxDep rs) (Vis op i k : IT _ A) σ ≡ (σ', Tau $ o))%I.
+    {A} `{!Cofe A} op i k o σ σ' th :
+    (gReifiers_re CtxDep rs op (i, σ, k) ≡ Some (o,σ',th)
+     ⊢@{iProp} reify (sr CtxDep rs) (Vis op i k : IT _ A) σ ≡ (σ', Tau $ o, listO_map Tau th))%I.
   Proof.
     apply uPred.internal_eq_entails=>m.
     intros H. apply reify_vis_dist_ctx_dep. exact H.
   Qed.
 
   Lemma reify_vis_eqI_ctx_indep (rs : gReifiers NotCtxDep sz)
-    {A} `{!Cofe A} op i k o σ σ' :
-    (gReifiers_re NotCtxDep rs op (i, σ) ≡ Some (o,σ')
-     ⊢@{iProp} reify (sr NotCtxDep rs) (Vis op i k : IT _ A) σ ≡ (σ', Tau $ k o))%I.
+    {A} `{!Cofe A} op i k o σ σ' th :
+    (gReifiers_re NotCtxDep rs op (i, σ) ≡ Some (o,σ',th)
+     ⊢@{iProp} reify (sr NotCtxDep rs) (Vis op i k : IT _ A) σ ≡ (σ', Tau $ k o, listO_map Tau th))%I.
   Proof.
     apply uPred.internal_eq_entails=>m.
     intros H. apply reify_vis_dist_ctx_indep. exact H.
@@ -488,12 +492,12 @@ Section greifiers.
     (x : Ins (sReifier_ops _ op) ♯ X)
     (y : laterO X)
     (k : (Outs (sReifier_ops r op) ♯ X -n> laterO X))
-    (s1 s2 : sReifier_state r ♯ X) :
-    sReifier_re r op (x, s1, k) ≡ Some (y, s2)
+    (s1 s2 : sReifier_state r ♯ X) th :
+    sReifier_re r op (x, s1, k) ≡ Some (y, s2, th)
     ⊢@{iProp}
        sReifier_re  (rs !!! sR_idx) (subEff_opid op)
        (subEff_ins x, sR_state s1, k ◎ (subEff_outs ^-1)) ≡
-       Some (y, sR_state s2).
+       Some (y, sR_state s2, th).
   Proof.
     apply uPred.internal_eq_entails=>m.
     intros H'.
@@ -507,12 +511,12 @@ Section greifiers.
     `{!@subReifier sz NotCtxDep r rs} {X} `{!Cofe X} (op : opid (sReifier_ops r))
     (x : Ins (sReifier_ops _ op) ♯ X)
     (y : Outs (sReifier_ops _ op) ♯ X)
-    (s1 s2 : sReifier_state r ♯ X) :
-    sReifier_re r op (x, s1) ≡ Some (y, s2)
+    (s1 s2 : sReifier_state r ♯ X) th :
+    sReifier_re r op (x, s1) ≡ Some (y, s2, th)
     ⊢@{iProp}
        sReifier_re (rs !!! sR_idx) (subEff_opid op)
        (subEff_ins x, sR_state s1) ≡
-       Some (subEff_outs y, sR_state s2).
+       Some (subEff_outs y, sR_state s2, th).
   Proof.
     apply uPred.internal_eq_entails=>m.
     apply (@sR_re _ NotCtxDep).
@@ -523,12 +527,12 @@ Section greifiers.
     (op : opid (sReifier_ops r))
     (x : Ins (sReifier_ops _ op) ♯ X) (y : laterO X)
     (k : (Outs (sReifier_ops r op) ♯ X -n> laterO X))
-    (σ σ' : sReifier_state r ♯ X) (rest : gState_rest CtxDep sR_idx rs ♯ X) :
-    sReifier_re r op (x,σ, k) ≡ Some (y, σ')
+    (σ σ' : sReifier_state r ♯ X) (rest : gState_rest CtxDep sR_idx rs ♯ X) th :
+    sReifier_re r op (x,σ, k) ≡ Some (y, σ', th)
     ⊢@{iProp}
        gReifiers_re CtxDep rs (subEff_opid op)
        (subEff_ins x, gState_recomp CtxDep rest (sR_state σ), k ◎ (subEff_outs ^-1))
-       ≡ Some (y, gState_recomp CtxDep rest (sR_state σ')).
+       ≡ Some (y, gState_recomp CtxDep rest (sR_state σ'), th).
   Proof.
     apply uPred.internal_eq_entails=>m.
     intros He.
@@ -542,12 +546,12 @@ Section greifiers.
     `{!@subReifier sz NotCtxDep r rs} {X} `{!Cofe X}
     (op : opid (sReifier_ops r))
     (x : Ins (sReifier_ops _ op) ♯ X) (y : Outs (sReifier_ops _ op) ♯ X)
-    (σ σ' : sReifier_state r ♯ X) (rest : gState_rest NotCtxDep sR_idx rs ♯ X) :
-    sReifier_re r op (x,σ) ≡ Some (y, σ')
+    (σ σ' : sReifier_state r ♯ X) (rest : gState_rest NotCtxDep sR_idx rs ♯ X) th :
+    sReifier_re r op (x,σ) ≡ Some (y, σ', th)
     ⊢@{iProp}
        gReifiers_re NotCtxDep rs (subEff_opid op)
        (subEff_ins x, gState_recomp NotCtxDep rest (sR_state σ))
-       ≡ Some (subEff_outs y, gState_recomp NotCtxDep rest (sR_state σ')).
+       ≡ Some (subEff_outs y, gState_recomp NotCtxDep rest (sR_state σ'), th).
   Proof.
     apply uPred.internal_eq_entails=>m.
     intros He.
@@ -557,16 +561,17 @@ Section greifiers.
     simpl in J.
     simpl.
     rewrite J//; clear J.
-    transitivity (prod_map (λ x0 : Outs (sReifier_ops (rs !!! sR_idx)
+    transitivity (prod_map (prod_map (λ x0 : Outs (sReifier_ops (rs !!! sR_idx)
                                            (subEff_opid op)) ♯ X, x0)
                     (λ st : sReifier_state (rs !!! sR_idx) ♯ X,
-                        (gState_decomp' NotCtxDep sR_idx rs ^-1) (st, rest)) <$>
+                        (gState_decomp' NotCtxDep sR_idx rs ^-1) (st, rest))) idfun <$>
                     (Some
-                       (subEff_outs y, sR_state σ'))).
+                       (subEff_outs y, sR_state σ', th))).
     - unfold prod_map.
       rewrite option_fmap_ne; [reflexivity | intros ??? | apply He].
-      do 2 f_equiv; first assumption.
-      do 2 f_equiv; assumption.
+      f_equiv; last (simpl; by f_equiv).
+      f_equiv; first (by do 2 f_equiv).
+      by do 4 f_equiv.
     - simpl.
       reflexivity.
   Qed.
