theories/lib/eq.v
@@ -1,0 +1,365 @@
+From gitrees Require Import prelude.
+From gitrees Require Import gitree.
+From iris.algebra Require Import list.
+
+Section ofe_decision.
+  Class Ofe_decide_eq (R : ofe) :=
+    MkOfeDecide {
+        ofe_decision : R -n> R -n> boolO;
+        ofe_decision_reflect : ∀ a b, ofe_decision a b = true -> a ≡ b;
+      }.
+  Arguments MkOfeDecide {_}.
+
+  Global Program Instance ofe_decide_eq_nat : Ofe_decide_eq natO
+    := MkOfeDecide (λne x y, Nat.eqb x y) _.
+  Next Obligation.
+    intros; simpl in *.
+    rewrite Nat.eqb_eq in H.
+    done.
+  Qed.
+  Fail Next Obligation.
+
+  Global Program Instance ofe_decide_eq_unit : Ofe_decide_eq unitO
+    := MkOfeDecide (λne x y, true) _.
+  Next Obligation.
+    intros a b; simpl in *.
+    by destruct a, b.
+  Qed.
+  Fail Next Obligation.
+
+  Global Program Instance ofe_decide_eq_bool : Ofe_decide_eq boolO
+    := MkOfeDecide (λne x y, Bool.eqb x y) _.
+  Next Obligation.
+    intros; simpl in *.
+    by apply eqb_prop in H.
+  Qed.
+  Fail Next Obligation.
+
+  Global Instance forallb_ne {A : ofe} n :
+    Proper ((dist n) ==> (dist n) ==> dist n) (λ f : A -n> boolO, @forallb A f).
+  Proof.
+    intros x y Hxy a.
+    induction a as [| a1 a2 IH].
+    - intros [| b1 b2] Hab; first done.
+      inversion Hab.
+    - intros [| b1 b2] Hab; first inversion Hab.
+      simpl.
+      f_equiv.
+      + inversion Hab; subst.
+        rewrite (Hxy a1).
+        by f_equiv.
+      + inversion Hab; subst.
+        apply IH.
+        done.
+  Qed.
+
+  Global Program Instance ofe_decide_eq_list `{!Ofe_decide_eq R} : Ofe_decide_eq (listO R)
+    := MkOfeDecide
+         (λne x y, Nat.eqb (length x) (length y)
+                   && forallb (λne x, ofe_decision (fstO x) (snd x)) (zip_with (λ a b, (a, b)) x y))
+         _.
+  Next Obligation. solve_proper. Qed.
+  Next Obligation.
+    intros R ? x n l l' Hl.
+    f_equiv.
+    {
+      f_equiv.
+      by apply List.Forall2_length in Hl.
+    }
+    apply forallb_ne; last solve_proper.
+    intros [? ?]; simpl; solve_proper.
+  Qed.
+  Next Obligation.
+    intros R ? n l l' Hl y; simpl.
+    f_equiv.
+    - f_equiv.
+      by apply List.Forall2_length in Hl.
+    - unshelve epose proof
+        (@forallb_ne (prodO R R) n (λne x : prodO R R, ofe_decision x.1 x.2)
+           (λne x : prodO R R, ofe_decision x.1 x.2) (reflexivity _));
+        [apply _ | solve_proper |].
+      simpl in H.
+      apply H.
+      solve_proper.
+  Qed.
+  Next Obligation.
+    intros R ? a; simpl in *.
+    induction a as [| a1 a2 IH].
+    - intros [| b1 b2]; first done.
+      inversion 1.
+    - intros [| b1 b2]; first inversion 1.
+      rewrite andb_true_iff.
+      intros [H1 H2].
+      simpl in H1.
+      simpl in H2.
+      rewrite andb_true_iff in H2.
+      destruct H2 as [H2 H3].
+      apply ofe_decision_reflect in H2.
+      rewrite H2.
+      f_equiv.
+      apply IH.
+      apply andb_true_iff.
+      rewrite H1 H3.
+      done.
+  Qed.
+  Fail Next Obligation.
+
+  Global Program Instance ofe_decide_eq_sum {A B : ofe}
+    {H1 : Ofe_decide_eq A}
+    {H2 : Ofe_decide_eq B}
+    : Ofe_decide_eq (sumO A B)
+    := MkOfeDecide
+         (λne x y, match x with
+                   | inl x' =>
+                       match y with
+                       | inl y' => ofe_decision x' y'
+                       | inr _ => false
+                       end
+                   | inr x' =>
+                       match y with
+                       | inl _ => false
+                       | inr y' => ofe_decision x' y'
+                       end
+                   end) _.
+  Next Obligation.
+    intros A B ?? [x1 | x2] n [y1 | y2] [z1 | z2] H; simpl;
+      inversion H; subst; solve_proper.
+  Qed.
+  Next Obligation.
+    intros A B ?? n [x1 | x2] [y1 | y2] H; simpl;
+      inversion H; subst; intros [z1 | z2]; simpl;
+      solve_proper.
+  Qed.
+  Next Obligation.
+    intros A B ?? [x1 | x2] [y1 | y2] H; simpl in *.
+    - f_equiv.
+      by apply ofe_decision_reflect.
+    - by exfalso.
+    - by exfalso.
+    - f_equiv.
+      by apply ofe_decision_reflect.
+  Qed.
+  Fail Next Obligation.
+
+End ofe_decision.
+
+Arguments MkOfeDecide {_}.
+
+Section decidable_equality.
+  Context {A} `{AC : !Cofe A}.
+  Context {E : opsInterp}.
+  Notation IT := (IT E A).
+  Notation ITV := (ITV E A).
+
+  Context `{!invGS_gen hlc Σ}.
+  Notation iProp := (iProp Σ).
+
+  Context `{SO : !SubOfe natO A}.
+  Context {dec : Ofe_decide_eq A}.
+
+  Program Definition safe_compare_def
+    : IT -> IT -> IT := λ a b,
+      (get_val
+         (λne v2,
+           get_val
+             (λne v1,
+               get_ret2 (λne x y, Ret (if (ofe_decision x y) then 1 else 0)) v2 v1)
+             b) a).
+  Next Obligation.
+    intros ????? n.
+    intros ?? H.
+    f_equiv.
+    by rewrite H.
+  Qed.
+  Next Obligation.
+    intros ???? n.
+    intros x y H z; simpl.
+    f_equiv.
+    assert (ofe_decision x z ≡{n}≡ ofe_decision y z) as ->; first solve_proper.
+    done.
+  Qed.
+  Next Obligation.
+    intros ??? n.
+    intros ?? H.
+    by f_equiv.
+  Qed.
+  Next Obligation.
+    intros ?? n.
+    intros ?? H.
+    do 2 f_equiv; simpl.
+    intros ?; simpl.
+    by f_equiv.
+  Qed.
+
+  Global Instance safe_compare_ne' n :
+    Proper ((dist n) ==> (dist n) ==> (dist n)) safe_compare_def.
+  Proof.
+    intros a1 a2 Ha b1 b2 Hb.
+    solve_proper_prepare.
+    f_equiv; last done.
+    f_equiv; intros ?; simpl.
+    by f_equiv.
+  Qed.
+  Global Instance safe_compare_proper' :
+    Proper ((≡) ==> (≡) ==> (≡)) safe_compare_def.
+  Proof.
+    intros a1 a2 Ha b1 b2 Hb.
+    solve_proper_prepare.
+    f_equiv; last done.
+    f_equiv; intros ?; simpl.
+    by f_equiv.
+  Qed.
+
+  Program Definition safe_compare
+    : IT -n> IT -n> IT := λne a b, safe_compare_def a b.
+  Solve All Obligations with solve_proper.
+
+  Lemma safe_compare_reflect x y : safe_compare x y ≡ Ret 1 → x ≡ y.
+  Proof using A AC SO dec Σ.
+    destruct (IT_dont_confuse x)
+      as [[e Ha] | [[m Ha] | [ [g Ha] | [[α' Ha]|[op [i [ko Ha]]]] ]]].
+    - intros H.
+      rewrite /safe_compare /= Ha in H.
+      rewrite /safe_compare_def get_val_err in H.
+      exfalso.
+      symmetry in H.
+      assert (⊢@{iProp} False)%I; last by eapply uPred.pure_soundness.
+      iApply IT_ret_err_ne.
+      rewrite <-H.
+      done.
+    - intros H.
+      rewrite /safe_compare /= Ha in H.
+      rewrite /safe_compare_def in H.
+      destruct (IT_dont_confuse y)
+        as [[e' Ha'] | [[m' Ha'] | [ [g' Ha'] | [[α'' Ha']|[op' [i' [ko' Ha']]]] ]]].
+      + rewrite core.get_val_ret /= in H.
+        rewrite Ha' in H.
+        rewrite get_val_err in H.
+        exfalso.
+        assert (⊢@{iProp} False)%I; last by eapply uPred.pure_soundness.
+        iApply IT_ret_err_ne.
+        rewrite ->H.
+        done.
+      + rewrite core.get_val_ret /= in H.
+        rewrite Ha' in H.
+        rewrite core.get_val_ret /= in H.
+        rewrite core.get_ret_ret /= in H.
+        rewrite core.get_ret_ret /= in H.
+        destruct (ofe_decision m m') eqn:Heq.
+        * apply ofe_decision_reflect in Heq.
+          rewrite Heq in Ha.
+          by rewrite -Ha' in Ha.
+        * exfalso.
+          assert (⊢@{iProp} False)%I; last by eapply uPred.pure_soundness.
+          iAssert (0 ≡ 1)%I as "%G".
+          {
+            iApply Ret_inj.
+            rewrite <-H.
+            done.
+          }
+          inversion G.
+      + rewrite core.get_val_ret /= in H.
+        rewrite Ha' in H.
+        rewrite get_val_fun /= in H.
+        rewrite core.get_ret_ret /= in H.
+        rewrite get_ret_fun /= in H.
+        exfalso.
+        assert (⊢@{iProp} False)%I; last by eapply uPred.pure_soundness.
+        iApply IT_ret_err_ne.
+        rewrite ->H.
+        done.
+      + rewrite core.get_val_ret /= in H.
+        rewrite Ha' in H.
+        rewrite get_val_tick /= in H.
+        exfalso.
+        assert (⊢@{iProp} False)%I; last by eapply uPred.pure_soundness.
+        iApply IT_ret_tick_ne.
+        rewrite ->H.
+        done.
+      + rewrite core.get_val_ret /= in H.
+        rewrite Ha' in H.
+        rewrite get_val_vis /= in H.
+        exfalso.
+        assert (⊢@{iProp} False)%I; last by eapply uPred.pure_soundness.
+        iApply IT_ret_vis_ne.
+        rewrite ->H.
+        done.
+    - intros H.
+      rewrite /safe_compare /= /safe_compare_def /= Ha get_val_fun /= in H.
+      destruct (IT_dont_confuse y)
+        as [[e' Ha'] | [[m' Ha'] | [ [g' Ha'] | [[α'' Ha']|[op' [i' [ko' Ha']]]] ]]].
+      + rewrite Ha' get_val_err in H.
+        exfalso.
+        assert (⊢@{iProp} False)%I; last by eapply uPred.pure_soundness.
+        iApply IT_ret_err_ne.
+        rewrite ->H.
+        done.
+      + rewrite Ha' core.get_val_ret /= in H.
+        rewrite get_ret_fun in H.
+        exfalso.
+        assert (⊢@{iProp} False)%I; last by eapply uPred.pure_soundness.
+        iApply IT_ret_err_ne.
+        rewrite ->H.
+        done.
+      + rewrite Ha' get_val_fun /= in H.
+        rewrite get_ret_fun in H.
+        exfalso.
+        assert (⊢@{iProp} False)%I; last by eapply uPred.pure_soundness.
+        iApply IT_ret_err_ne.
+        rewrite ->H.
+        done.
+      + rewrite Ha' get_val_tick /= in H.
+        exfalso.
+        assert (⊢@{iProp} False)%I; last by eapply uPred.pure_soundness.
+        iApply IT_ret_tick_ne.
+        rewrite ->H.
+        done.
+      + rewrite Ha' in H.
+        rewrite get_val_vis /= in H.
+        exfalso.
+        assert (⊢@{iProp} False)%I; last by eapply uPred.pure_soundness.
+        iApply IT_ret_vis_ne.
+        rewrite ->H.
+        done.
+    - intros H.
+      rewrite /safe_compare /= /safe_compare_def /= Ha get_val_tick /= in H.
+      exfalso.
+      assert (⊢@{iProp} False)%I; last by eapply uPred.pure_soundness.
+      iApply IT_ret_tick_ne.
+      rewrite ->H.
+      done.
+    - intros H.
+      rewrite /safe_compare /= /safe_compare_def /= Ha get_val_vis /= in H.
+      exfalso.
+      assert (⊢@{iProp} False)%I; last by eapply uPred.pure_soundness.
+      iApply IT_ret_vis_ne.
+      rewrite ->H.
+      done.
+  Qed.
+
+  Lemma safe_compare_ret x y : safe_compare (Ret x) (Ret y) ≡ Ret (if ofe_decision x y then 1 else 0).
+  Proof.
+    rewrite /safe_compare /= /safe_compare_def.
+    rewrite get_val_ret /= get_val_ret /= get_ret_ret /= get_ret_ret //=.
+  Qed.
+
+  Lemma safe_compare_tick_l x y : safe_compare (Tick x) y ≡ Tick (safe_compare x y).
+  Proof.
+    rewrite /safe_compare /= /safe_compare_def.
+    rewrite get_val_tick.
+    f_equiv.
+  Qed.
+
+  Lemma safe_compare_tick_r x `{!AsVal x} y : safe_compare x (Tick y) ≡ Tick (safe_compare x y).
+  Proof.
+    rewrite /safe_compare /= /safe_compare_def.
+    rewrite get_val_ITV /=.
+    rewrite get_val_tick.
+    f_equiv.
+    rewrite get_val_ITV /=.
+    f_equiv.
+  Qed.
+
+End decidable_equality.
+
+Arguments safe_compare {_ _ _ _ _}.
